PiLL/PiLL/Framework/SessionFidelity.lean
@@ -2,1047 +2,41 @@ import PiLL.Framework.Semantics.EnvStep
 import PiLL.Framework.Semantics.ProcStep
 import PiLL.Framework.Substitution
 
+-- TODO: Implement the following instead of having post condition on res in EnvStep
+-- NOTE: Not possible without knowning that l.i is disjoint form ℋ, which could be
+-- obtained from a ProcStep sidecondition, but that would require having this be used
+-- inside e.g. session_fidelity and not having it be a strictly stand alone property /
+-- lemma for EnvStep - This would also need to know the corresponding ProcStep and Typing.
+-- But could work as an auxiliary for session fidelity, not standalone for EnvStep.
+-- lemma EnvStep.Linearity_and_subset {𝒢 𝒢' : HyperEnv} {l : Lbl}
+--   (hlin : 𝒢.Linearity) (hES : 𝒢 -[l]->ₑ 𝒢') :
+--   𝒢'.Linearity ∧ (𝒢'.names ⊆ 𝒢.names ∪ l.i) := by
+--   induction hES
 
 
+-- FIXME: Fix TypingStep
+-- FIXME: Typing_preserves_proc_congr
+-- FIXME: Use NameSpaces instead of having e.g. HyperEnv._____ everywhere
 
 
 
 
+-- FIXME: Proof showing substitution avoids capture
+-- FIXME: Proof showing AlphaEq is equivalent to = between Procs
+-- FIXME: Find different syntax for open?
+-- FIXME: Prove name substitution only being applied to free names?
 
 
+-- NOTE: shows the proof lean found using the simp_all tactic show_term { simp_all }
 
+-- FIXME: Move everything related to HyperEnv.Perm to a separate file? Or at least organize
+-- definition and lemma ordering a bit.
 
 
 
 
--- FIXME: Move to Proc
-@[simp] lemma Proc.f_nil :
-  𝟘.f = ∅ := by simp [Proc.f]
 
-@[simp] lemma Proc.f_one {P : Proc} {u : Channel} :
-  (u⟦⟧․P).f = u.f ∪ P.f := by simp [Proc.f]
-
-@[simp] lemma Proc.f_bot {P : Proc} {u : Channel} :
-  (u⸨⸩․P).f = u.f ∪ P.f := by simp [Proc.f]
-
-@[simp] lemma Proc.f_tensor {P : Proc} {u : Channel} :
-  (u⟦$N⟧․P).f = u.f ∪ P.f := by simp [Proc.f]
-
-@[simp] lemma Proc.f_parr {P : Proc} {u : Channel} :
-  (u⸨$N⸩․P).f = u.f ∪ P.f := by simp [Proc.f]
-
-@[simp] lemma Proc.f_cut {P : Proc} :
-  (𝑣⸨$N,$N⸩ P).f = P.f := by simp [Proc.f]
-
-@[simp] lemma Proc.f_par {P Q : Proc} :
-   (P |ₚ Q).f = P.f ∪ Q.f := by simp [Proc.f]
-
-@[simp] lemma Proc.f_selectL {P : Proc} {u : Channel} :
-  (u⟦𝐋⟧․P).f = u.f ∪ P.f := by simp [Proc.f]
-
-@[simp] lemma Proc.f_selectR {P : Proc} {u : Channel} :
-  (u⟦𝐑⟧․P).f = u.f ∪ P.f := by simp [Proc.f]
-
-@[simp] lemma Proc.f_amp {P Q : Proc} {u : Channel} :
-  (u․case{𝐋 : P, 𝐑 : Q}).f = u.f ∪ P.f ∪ Q.f := by simp [Proc.f]
-
-@[simp] lemma Proc.f_output {P : Proc} {u : Channel} {A : Types} :
-  (u⟦A⟧․P).f = u.f ∪ P.f := by simp [Proc.f]
-
-@[simp] lemma Proc.f_input {P : Proc} {u : Channel} :
-  (u⸨$T⸩․P).f = u.f ∪ P.f := by simp [Proc.f]
-
-@[simp] lemma Proc.f_server {P : Proc} {u : Channel} :
-  (!u․{P}).f = u.f ∪ P.f := by simp [Proc.f]
-
-@[simp] lemma Proc.f_consume {P : Proc} {u : Channel} :
-  (u⟦USE⟧․P).f = u.f ∪ P.f := by simp [Proc.f]
-
-@[simp] lemma Proc.f_duplicate {P : Proc} {u : Channel} :
-  (u⟦DUP⟧⸨$N⸩․P).f = u.f ∪ P.f := by simp [Proc.f]
-
-@[simp] lemma Proc.f_dispose {P : Proc} {u : Channel} :
-  (u⟦DISP⟧․P).f = u.f ∪ P.f := by simp [Proc.f]
-
-@[simp] lemma Proc.f_link {u v : Channel} :
-  (u⟷ₚv).f = u.f ∪ v.f := by simp [Proc.f]
-
-
-@[simp] lemma Channel.f_open_erase {k : Nat} {u : Channel} {y : FPName} (hy : y ∉ u.f) :
-  (u⸨k | #y⸩).f.erase y = u.f := by
-  cases u with
-  | bound =>
-    simp [HasOpen.open_, Channel.open, Channel.f]
-    split_ifs <;> simp
-  | free z =>
-    simp [HasOpen.open_, Channel.open, Channel.f] at ⊢ hy
-    exact hy
-
-@[simp] lemma Proc.f_open_erase {P : Proc} {y : FPName} {k : Nat} (hy : y ∉ P.f) :
-  (P⸨k | #y⸩.f).erase y = P.f := by
-  induction P generalizing k <;> simp [Finset.erase_union_distrib] at ⊢ hy
-
-  case one ih | bot ih | tensor ih | parr ih | selectL ih | selectR ih | output ih | input ih
-    | server ih | consume ih | duplicate ih | dispose ih =>
-    rw [Channel.f_open_erase hy.1, ih hy.2]
-
-  case cut ih => exact ih hy
-  case par ihP ihQ => rw [ihP hy.1, ihQ hy.2]
-  case amp ihP ihQ => rw [Channel.f_open_erase hy.1, ihP hy.2.1, ihQ hy.2.2]
-  case link => rw [Channel.f_open_erase hy.1, Channel.f_open_erase hy.2]
-
-@[simp] lemma Proc.f_open_two_erase {P : Proc} {x y : FPName} {k : Nat}
-  (hx : x ∉ P.f) (hy : y ∉ P.f) (hneq : x ≠ y) :
-  ((P⸨k | #x, #y⸩.f).erase x).erase y = P.f := by
-  simp [HasOpenTwo.open_]
-  change (P⸨k + 1 | #y⸩⸨k | #x⸩.f.erase x).erase y = P.f
-  rw [Proc.f_open_erase, Proc.f_open_erase hy]
-  intro h
-  have h1 : (P⸨k + 1 | #y⸩.f).erase y = P.f := Proc.f_open_erase hy
-  have h2 := Finset.mem_erase_of_ne_of_mem hneq h
-  rw [h1] at h2
-  contradiction
-
-
-
-
-
-
-
-
-
-
-
--- FIXME: Move to Judgement
-lemma Typing.f_eq_names {n : Nat} {P : Proc} {𝒢 : HyperEnv} :
-  (n ⊢ P ∷ 𝒢) → P.f = 𝒢.names := by
-  intro h
-  induction h <;> try simp [Channel.f]
-
-  case mix ih1 ih2 => rw [ih1, ih2]
-
-  case one ih | bot ih | oplus₁ ih | oplus₂ ih | quest ih | bang ih | w ih | exists_ ih
-    | forall_ ih =>
-    simp [ih]
-
-  case cut ℋ Γ Δ P _ _ L _ ih =>
-    have ⟨x, y, hx, hy, hneq⟩ := exists_two_fresh (L ∪ P.f ∪ ℋ.names ∪ Γ.names ∪ Δ.names)
-    simp at hx hy ih
-    obtain ⟨hx1, hx2, hx3⟩ := hx
-    obtain ⟨hy1, hy2, hy3⟩ := hy
-    have := ih x y hx1 hy1 hneq
-    apply_fun (fun s => (s.erase y).erase x) at this
-    rw [Finset.erase_insert (by simp [hy3, hneq.symm]), Finset.erase_insert (by simp [hx3]),
-      Finset.erase_right_comm, Proc.f_open_two_erase hx2 hy2 hneq] at this
-    exact this
-
-  case tensor Γ Δ P x _ _ _ _ L _ ih =>
-    obtain ⟨y, hy⟩ := exists_one_fresh (L ∪ P.f ∪ {x} ∪ Γ.names ∪ Δ.names)
-    simp at hy ih
-    obtain ⟨hneq, hy1, hy2, hy3⟩ := hy
-    have := ih y hy1
-    apply_fun (fun s => s.erase y) at this
-    rw [Proc.f_open_erase hy2, Finset.insert_comm,
-      Finset.erase_insert (by simp [hneq, hy3])] at this
-    simp [this]
-
-  case parr Γ P x _ _ _ _ L _ ih =>
-    obtain ⟨y, hy⟩ := exists_one_fresh (L ∪ P.f ∪ {x} ∪ Γ.names)
-    simp at hy ih
-    obtain ⟨hneq, hy1, hy2, hy3⟩ := hy
-    have := ih y hy1
-    apply_fun (fun s => s.erase y) at this
-    rw [Proc.f_open_erase hy2, Finset.insert_comm,
-      Finset.erase_insert (by simp [hneq, hy3])] at this
-    simp [this]
-
-  case c Γ P x _ _ _ L _ ih =>
-    obtain ⟨y, hy⟩ := exists_one_fresh (L ∪ P.f ∪ {x} ∪ Γ.names)
-    simp at hy ih
-    obtain ⟨hneq, hy1, hy2, hy3⟩ := hy
-    have := ih y hy1
-    apply_fun (fun s => s.erase y) at this
-    rw [Proc.f_open_erase hy2, Finset.erase_insert (by simp [hneq, hy3])] at this
-    simp [this]
-
-  case amp ihP ihQ => simp [ihP, ihQ]
-
-  case exchange_env hP ih =>
-    simp [ih, Env.names_eq_of_perm hP]
-
-  case exchange_hyper hP ih =>
-    simp [ih, HyperEnv.names_eq_of_perm hP]
-
-@[simp] lemma Env.swap_two {x y : FPName} {A B : Types} :
-  [x ∶ A, y ∶ B] ~ [y ∶ B, x ∶ A] := by
-  exact List.Perm.swap ..
-
-
--- FIXME: use this (HyperEnv.Perm.trans hP HyperEnv.swap_two_inner) for comm?
-@[simp] lemma HyperEnv.swap_two_inner {x y : FPName} {A B : Types} :
-  [[x ∶ A, y ∶ B]] ~ [[y ∶ B, x ∶ A]] := by
-  exact HyperEnv.Perm.cons Env.swap_two HyperEnv.Perm.nil
-
-@[simp] lemma HyperEnv.disjoint_split {𝒢 ℋ : HyperEnv} (hD : (𝒢 |ₕ ℋ).PairwiseDisjoint) :
-  𝒢.disjoint ℋ := by
-  rw [HyperEnv.disjoint, Finset.disjoint_left]
-  rw [HyperEnv.PairwiseDisjoint, HyperEnv.merge, List.pairwise_append] at hD
-  intro n hin𝒢 hinℋ
-  rw [HyperEnv.mem_pair_fst_in_names] at hin𝒢 hinℋ
-  obtain ⟨T1, Γ, hinΓ, hΓ𝒢⟩ := hin𝒢
-  obtain ⟨T2, Δ, hinΔ, hΔℋ⟩ := hinℋ
-  obtain ⟨h1, h2, h3⟩ := hD
-  have := h3 Γ hΓ𝒢 Δ hΔℋ
-  simp [Env.disjoint] at this
-  have hnΓ := Env.mem_pair_fst_in_names T1 hinΓ
-  have hnΔ := Env.mem_pair_fst_in_names T2 hinΔ
-  rw [Finset.disjoint_left] at this
-  exact this hnΓ hnΔ
-
-
-
-
-
-lemma Typing_inv_one {n : Nat} {P : Proc} {x : FPName} {𝒢 : HyperEnv}
-  (hT : Typing n (#x⟦⟧․P) 𝒢) :
-  (𝒢 ~ [[x ∶ 1]]) ∧ Typing n P ∅ := by
-  generalize heq : (#x⟦⟧․P) = P' at hT
-  induction hT generalizing P x <;> try contradiction
-
-  case exchange_env ℋ _ _ _ _ _ hP ih =>
-    have ⟨h1, h2⟩ := ih heq
-    have := HyperEnv.Perm.cons hP.symm (HyperEnv.Perm.refl ℋ)
-    exact ⟨HyperEnv.Perm.trans this h1, h2⟩
-
-  case exchange_hyper hP ih =>
-    have ⟨h1, h2⟩ := ih heq
-    exact ⟨HyperEnv.Perm.trans hP.symm h1, h2⟩
-
-  case one hT _ =>
-    simp at heq
-    constructor
-    · simp [heq.1, HasPerm.perm]
-    · simp [heq.2]
-      exact hT
-
-lemma Typing_inv_bot {n : Nat} {P : Proc} {x : FPName} {𝒢 : HyperEnv}
-  (hT : Typing n (#x⸨⸩․P) 𝒢) :
-  ∃ Γ, (𝒢 ~ [x ∶ ⊥ :: Γ]) ∧ Typing n P [Γ] := by
-  generalize heq : (#x⸨⸩․P) = P' at hT
-  induction hT generalizing P x <;> try contradiction
-
-  case exchange_env ℋ _ _ _ _ _ hP ih =>
-    have ⟨Ξ, h⟩ := ih heq
-    obtain ⟨h1, h2⟩ := h
-    constructor
-    · have := HyperEnv.Perm.cons hP.symm (HyperEnv.Perm.refl ℋ)
-      exact ⟨HyperEnv.Perm.trans this h1, h2⟩
-
-  case exchange_hyper hP ih =>
-    have ⟨Γ, h⟩ := ih heq
-    obtain ⟨h1, h2⟩ := h
-    constructor
-    · exact ⟨HyperEnv.Perm.trans hP.symm h1, h2⟩
-
-  case bot hT _ =>
-    simp at heq
-    constructor
-    · constructor
-      · simp [heq.1]
-        apply HyperEnv.Perm.refl
-      · simp [heq.2]
-        exact hT
-
-lemma Typing_inv_tensor {n : Nat} {P : Proc} {𝒢 : HyperEnv} {x : FPName}
-  (hT : Typing n (#x⟦$N⟧․P) 𝒢) :
-  ∃ (A B : Types) (Γ Δ : Env) (L : Finset FPName),
-    (𝒢 ~ [x ∶ A ⨂ B :: Γ‚ Δ]) ∧ (∀ z ∉ L, Typing n (P⸨#z⸩) ([z ∶ A :: Γ] |ₕ [x ∶ B :: Δ])) := by
-  generalize heq : (#x⟦$N⟧․P) = P' at hT
-  induction hT generalizing P <;> try contradiction
-
-  case exchange_env hP ih =>
-    obtain ⟨A, B, Γ, Δ, L, hP', hT'⟩ := ih heq
-    use A, B, Γ, Δ, L
-    constructor
-    · exact (HyperEnv.Perm.trans (hP'.symm) (HyperEnv.Perm.cons hP (HyperEnv.Perm.refl _))).symm
-    · exact hT'
-
-  case exchange_hyper hP ih =>
-    obtain ⟨A, B, Γ, Δ, L, hP', hT'⟩ := ih heq
-    use A, B, Γ, Δ, L
-    constructor
-    · exact HyperEnv.Perm.trans (hP.symm) hP'
-    · exact hT'
-
-  case tensor Γ Δ Q _ A B _ _ L hT ih =>
-    obtain ⟨z, hz⟩ := exists_one_fresh (L ∪ Γ.names ∪ Δ.names ∪ Q.f ∪ {x})
-    simp at hz heq
-    obtain ⟨hz1, hz2, hz3, hz4, hz5⟩ := hz
-    use A, B, Γ, Δ, L
-    constructor
-    · rw [heq.1]
-    · rw [heq.1, heq.2]
-      exact hT
-
-lemma Typing_inv_parr {n : Nat} {P : Proc} {𝒢 : HyperEnv} {x : FPName}
-  (hT : Typing n (#x⸨$N⸩․P) 𝒢) :
-  ∃ (A B : Types) (Γ : Env) (L : Finset FPName),
-    (𝒢 ~ [x ∶ A ⅋ B :: Γ]) ∧ (∀ z ∉ L, Typing n (P⸨#z⸩) ([z ∶ A :: x ∶ B :: Γ])) := by
-  generalize heq : (#x⸨$N⸩․P) = P' at hT
-  induction hT generalizing P <;> try contradiction
-
-  case exchange_env hP ih =>
-    obtain ⟨A, B, Γ, L, hP', hT'⟩:= ih heq
-    use A, B, Γ, L
-    constructor
-    · exact (HyperEnv.Perm.trans (hP'.symm) (HyperEnv.Perm.cons hP (HyperEnv.Perm.refl _))).symm
-    · exact hT'
-
-  case exchange_hyper hP ih =>
-    obtain ⟨A, B, Γ, L, hP', hT'⟩ := ih heq
-    use A, B, Γ, L
-    constructor
-    · exact HyperEnv.Perm.trans (hP.symm) hP'
-    · exact hT'
-
-  case parr Γ Q y A B hF n L hT ih =>
-    obtain ⟨z, hz⟩ := exists_one_fresh (L ∪ Γ.names ∪ Q.f ∪ {x})
-    simp at hz heq
-    obtain ⟨hz1, hz2, hz3, hz4⟩ := hz
-    use A, B, Γ, L
-    constructor
-    · rw [heq.1]
-    · rw [heq.1, heq.2]
-      exact hT
-
-lemma Typing_inv_par {n : Nat} {P Q : Proc} {𝒢 : HyperEnv} (hT : n ⊢ P |ₚ Q ∷ 𝒢) :
-  ∃ 𝒢₁ 𝒢₂, (𝒢 ~ 𝒢₁ |ₕ 𝒢₂) ∧ (n ⊢ P ∷ 𝒢₁) ∧ (n ⊢ Q ∷ 𝒢₂) := by
-  generalize heq : (P |ₚ Q) = PQ at hT
-  induction hT generalizing P Q <;> try contradiction
-
-  case exchange_env hP ih =>
-    obtain ⟨ℋ₁, ℋ₂, hP', hT'⟩ := ih heq
-    use ℋ₁, ℋ₂
-    constructor
-    · exact HyperEnv.Perm.trans (HyperEnv.Perm.cons hP.symm (HyperEnv.Perm.refl _)) hP'
-    · exact hT'
-
-  case exchange_hyper hP ih =>
-    obtain ⟨ℋ₁, ℋ₂, hP', hT'⟩ := ih heq
-    use ℋ₁, ℋ₂
-    constructor
-    · exact HyperEnv.Perm.trans hP.symm hP'
-    · exact hT'
-
-  case mix 𝒢 ℋ _ _ hD _ hTP hTQ ihP ihQ =>
-    simp at heq
-    obtain ⟨hP, hQ⟩ := heq
-    use 𝒢, ℋ
-    rw [hP, hQ]
-    exact ⟨by simp, ⟨hTP, hTQ⟩⟩
-
-lemma Typing_inv_link {n : Nat} {x y : FPName} {𝒢 : HyperEnv}
-  (hT : n ⊢ #x⟷ₚ#y ∷ 𝒢) :
-  ∃ A, 𝒢 ~ [x ∶ Aᗮ :: [y ∶ A]] := by
-  generalize heq : (#x⟷ₚ#y) = P at hT
-  induction hT generalizing x y <;> try contradiction
-
-  case exchange_env hP ih =>
-    obtain ⟨T, hP'⟩ := ih heq
-    use T
-    exact HyperEnv.Perm.trans (HyperEnv.Perm.cons hP.symm HyperEnv.Perm.rfl) hP'
-
-  case exchange_hyper hP ih =>
-    obtain ⟨T, hP'⟩ := ih heq
-    use T
-    exact HyperEnv.Perm.trans hP.symm hP'
-
-  case ax A _ hneq hlc =>
-    simp at heq
-    obtain ⟨rfl, rfl⟩ := heq
-    use A
-
-lemma Typing_inv_amp {n : Nat} {x : FPName} {P Q : Proc} {𝒢 : HyperEnv}
-  (hT : n ⊢ #x․case{𝐋 : P, 𝐑 : Q} ∷ 𝒢) :
-  ∃ Γ A B, (𝒢 ~ [x ∶ A & B :: Γ]) ∧ (n ⊢ P ∷ [x ∶ A :: Γ]) ∧ (n ⊢ Q ∷ [x ∶ B :: Γ]) := by
-  generalize heq : (#x․case{𝐋 : P, 𝐑 : Q}) = PQ at hT
-  induction hT generalizing P Q x <;> try contradiction
-
-  case exchange_env hP ih =>
-    obtain ⟨𝒢', A, B, hP', hT'⟩ := ih heq
-    use 𝒢', A, B
-    constructor
-    · exact HyperEnv.Perm.trans (HyperEnv.Perm.cons hP.symm (HyperEnv.Perm.refl _)) hP'
-    · exact hT'
-
-  case exchange_hyper hP ih =>
-    obtain ⟨𝒢', A, B, hP', hT'⟩ := ih heq
-    use 𝒢', A, B
-    constructor
-    · exact HyperEnv.Perm.trans hP.symm hP'
-    · exact hT'
-
-  case amp Γ _ _ x A B _ hTP hTQ ihP ihQ =>
-    simp at heq
-    obtain ⟨rfl, rfl, rfl⟩ := heq
-    use Γ, A, B
-
-lemma Typing_inv_selectL {n : Nat} {x : FPName} {P : Proc} {𝒢 : HyperEnv}
-  (hT : n ⊢ #x⟦𝐋⟧․P ∷ 𝒢) :
-  ∃ Γ A B, (𝒢 ~ [x ∶ A ⊕ B :: Γ]) ∧ (n ⊢ P ∷ [x ∶ A :: Γ]) := by
-  generalize heq : (#x⟦𝐋⟧․P) = PsL at hT
-  induction hT generalizing P x <;> try contradiction
-
-  case exchange_env hP ih =>
-    obtain ⟨Γ, A, B, hP', hT'⟩ := ih heq
-    use Γ, A, B
-    constructor
-    · exact HyperEnv.Perm.trans (HyperEnv.Perm.cons hP.symm (HyperEnv.Perm.refl _)) hP'
-    · exact hT'
-
-  case exchange_hyper hP ih =>
-    obtain ⟨Γ, A, B, hP', hT'⟩ := ih heq
-    use Γ, A, B
-    constructor
-    · exact HyperEnv.Perm.trans hP.symm hP'
-    · exact hT'
-
-  case oplus₁ Γ _ _ A B  _ hlc hPT ih =>
-    simp at heq
-    obtain ⟨rfl, rfl⟩ := heq
-    use Γ, A, B
-
-lemma Typing_inv_selectR {n : Nat} {x : FPName} {P : Proc} {𝒢 : HyperEnv}
-  (hT : n ⊢ #x⟦𝐑⟧․P ∷ 𝒢) :
-  ∃ Γ A B, (𝒢 ~ [x ∶ A ⊕ B :: Γ]) ∧ (n ⊢ P ∷ [x ∶ B :: Γ]) := by
-  generalize heq : (#x⟦𝐑⟧․P) = PsR at hT
-  induction hT generalizing P x <;> try contradiction
-
-  case exchange_env hP ih =>
-    obtain ⟨Γ, A, B, hP', hT'⟩ := ih heq
-    use Γ, A, B
-    constructor
-    · exact HyperEnv.Perm.trans (HyperEnv.Perm.cons hP.symm (HyperEnv.Perm.refl _)) hP'
-    · exact hT'
-
-  case exchange_hyper hP ih =>
-    obtain ⟨Γ, A, B, hP', hT'⟩ := ih heq
-    use Γ, A, B
-    constructor
-    · exact HyperEnv.Perm.trans hP.symm hP'
-    · exact hT'
-
-  case oplus₂ Γ _ _ A B  _ hlc hPT ih =>
-    simp at heq
-    obtain ⟨rfl, rfl⟩ := heq
-    use Γ, A, B
-
-lemma Typing_inv_output {n : Nat} {x : FPName} {A : Types} {P : Proc} {𝒢 : HyperEnv}
-  (hT : n ⊢ #x⟦A⟧․P ∷ 𝒢) :
-  ∃ Γ B,
-  (𝒢 ~ [x ∶ ∃․B :: Γ]) ∧ n ⊢ P ∷ [x ∶ B{A // 0} :: Γ] := by
-  generalize heq : (#x⟦A⟧․P) = Pout at hT
-  induction hT generalizing P x <;> try contradiction
-
-  case exchange_env hP ih =>
-    obtain ⟨Γ, B, hP', hT'⟩ := ih heq
-    use Γ, B
-    constructor
-    · exact HyperEnv.Perm.trans (HyperEnv.Perm.cons hP.symm (HyperEnv.Perm.refl _)) hP'
-    · exact hT'
-
-  case exchange_hyper hP ih =>
-    obtain ⟨Γ, A, hP', hT'⟩ := ih heq
-    use Γ, A
-    constructor
-    · exact HyperEnv.Perm.trans hP.symm hP'
-    · exact hT'
-
-  case exists_ Γ _ _ _ B _ hlc hT ih =>
-    simp at heq
-    obtain ⟨rfl, rfl, rfl⟩ := heq
-    use Γ, B
-
-lemma Typing_inv_input {n : Nat} {x : FPName} {P : Proc} {𝒢 : HyperEnv}
-  (hT : n ⊢ #x⸨$T⸩․P ∷ 𝒢) :
-  ∃ (Γ : Env) (B : Types),
-  (𝒢 ~ [x ∶ ∀․B :: Γ]) ∧ (n + 1 ⊢ P ∷ [x ∶ B :: Γ⁺ᵗ]) := by
-  generalize heq : (#x⸨$T⸩․P) = Pin at hT
-  induction hT generalizing P x <;> try contradiction
-
-  case exchange_env hP ih =>
-    obtain ⟨Γ, B, hP', hT'⟩ := ih heq
-    use Γ, B
-    constructor
-    · exact HyperEnv.Perm.trans (HyperEnv.Perm.cons hP.symm (HyperEnv.Perm.refl _)) hP'
-    · exact hT'
-
-  case exchange_hyper hP ih =>
-    obtain ⟨Γ, B, hP', hT'⟩ := ih heq
-    use Γ, B
-    constructor
-    · exact HyperEnv.Perm.trans hP.symm hP'
-    · exact hT'
-
-  case forall_ Γ _ _ B _ _ ih  =>
-    simp at heq
-    obtain ⟨rfl, rfl⟩ := heq
-    use Γ, B
-
-lemma Typing_inv_use₁ {n : Nat} {x : FPName} {P : Proc} {𝒢 : HyperEnv}
-  (hT : n ⊢ #x⟦USE⟧․P ∷ 𝒢) :
-  ∃ Γ A, (𝒢 ~ [x ∶ ??A :: Γ]) ∧ (n ⊢ P ∷ [x ∶ A :: Γ]) := by
-  generalize heq : (#x⟦USE⟧․P) = Puse at hT
-  induction hT generalizing P x <;> try contradiction
-
-  case exchange_env 𝒢 _ _ _ _ _ hP ih =>
-    obtain ⟨Γ, A, hP', hT'⟩ := ih heq
-    use Γ, A
-    constructor
-    · exact HyperEnv.Perm.trans (HyperEnv.Perm.cons hP.symm (HyperEnv.Perm.refl 𝒢)) hP'
-    · exact hT'
-
-  case exchange_hyper hP ih =>
-    obtain ⟨Γ, A, hP', hT'⟩ := ih heq
-    use Γ, A
-    constructor
-    · exact HyperEnv.Perm.trans hP.symm hP'
-    · exact hT'
-
-  case quest Γ _ _ A _ _ ih =>
-    simp at heq
-    obtain ⟨rfl, rfl⟩ := heq
-    use Γ, A
-
-lemma Typing_inv_use₂ {n : Nat} {x : FPName} {P : Proc} {𝒢 : HyperEnv}
-  (hT : n ⊢ !#x․{P} ∷ 𝒢) :
-  ∃ Γ A, (𝒢 ~ [x ∶ !!A :: Γ]) ∧ (n ⊢ P ∷ [x ∶ A :: Γ]) ∧ ?ₑΓ := by
-  generalize heq : (!#x․{P}) = Puse at hT
-  induction hT generalizing P x <;> try contradiction
-
-  case exchange_env 𝒢 _ _ _ _ _ hP ih =>
-    obtain ⟨Γ, A, hP', hT'⟩ := ih heq
-    use Γ, A
-    constructor
-    · exact HyperEnv.Perm.trans (HyperEnv.Perm.cons hP.symm (HyperEnv.Perm.refl 𝒢)) hP'
-    · exact hT'
-
-  case exchange_hyper hP ih =>
-    obtain ⟨Γ, A, hP', hT'⟩ := ih heq
-    use Γ, A
-    constructor
-    · exact HyperEnv.Perm.trans hP.symm hP'
-    · exact hT'
-
-  case bang Γ _ _ A _ _ _ _ =>
-    simp at heq
-    obtain ⟨rfl, rfl⟩ := heq
-    use Γ, A
-
-lemma Typing_inv_disp₁ {n : Nat} {x : FPName} {P : Proc} {𝒢 : HyperEnv}
-  (hT : n ⊢ #x⟦DISP⟧․P ∷ 𝒢) :
-  ∃ Γ A, (𝒢 ~ [x ∶ ??A :: Γ]) ∧ (n ⊢ P ∷ [Γ]) ∧ x ∉ Env.names Γ := by
-  generalize heq : (#x⟦DISP⟧․P) = Pdisp at hT
-  induction hT generalizing P x <;> try contradiction
-
-  case exchange_env hP ih =>
-    obtain ⟨Γ, A, hP', hT'⟩ := ih heq
-    use Γ, A
-    constructor
-    · exact HyperEnv.Perm.trans (HyperEnv.Perm.cons hP.symm (HyperEnv.Perm.refl _)) hP'
-    · exact hT'
-
-  case exchange_hyper hP ih =>
-    obtain ⟨Γ, A, hP', hT'⟩ := ih heq
-    use Γ, A
-    constructor
-    · exact HyperEnv.Perm.trans hP.symm hP'
-    · exact hT'
-
-  case w Γ _ _ A _ _ _ _ _ =>
-    simp at heq
-    obtain ⟨rfl, rfl⟩ := heq
-    use Γ, A
-
-lemma Typing_inv_dup₁ {n : Nat} {x : FPName} {P : Proc} {𝒢 : HyperEnv}
-  (hT : n ⊢ #x⟦DUP⟧⸨$N⸩․P ∷ 𝒢) :
-  ∃ (Γ : Env) (A : Types) (L : Finset FPName),
-    (𝒢 ~ [x ∶ ??A :: Γ]) ∧ x ∉ Γ.names ∧
-    (∀ x' ∉ L, x' ≠ x → n ⊢ P⸨#x'⸩ ∷ [x' ∶ ??A :: x ∶ ??A :: Γ]) := by
-  generalize heq : (#x⟦DUP⟧⸨$N⸩․P) = Pdup at hT
-  induction hT generalizing P x <;> try contradiction
-
-  case exchange_env hP ih =>
-    obtain ⟨Γ, A, x', hP', hT'⟩ := ih heq
-    use Γ, A, x'
-    constructor
-    · exact HyperEnv.Perm.trans (HyperEnv.Perm.cons hP.symm (HyperEnv.Perm.refl _)) hP'
-    · exact hT'
-
-  case exchange_hyper hP ih =>
-    obtain ⟨Γ, A, x', hP', hT'⟩ := ih heq
-    use Γ, A, x'
-    constructor
-    · exact HyperEnv.Perm.trans hP.symm hP'
-    · exact hT'
-
-  case c Γ _ _ A _ hF L hT _ =>
-    simp at heq
-    obtain ⟨rfl, rfl⟩ := heq
-    use Γ, A, L
-    constructor
-    · simp
-    · constructor
-      · exact hF
-      · intros x' hin hneq
-        apply Typing.exchange_hyper (hT x' hin)
-        exact HyperEnv.Perm.cons (List.Perm.swap (x' ∶ ??A) (x ∶ ??A) Γ) (by simp)
-
-
-lemma Typing_buildDisp {n : Nat} {x : FPName} (Γ : Env) (names : List FPName)
-  (hServ : ?ₑΓ) (hNodup : names.Nodup) (heq : Γ.names = names.toFinset)
-  (hxΓ : x ∉ Γ.names) (hlc : Γ.lc n) (hNodupΓ : Env.Nodup Γ)
-  : n ⊢ buildDisp names x ∷ [x ∶ 1 :: Γ] := by
-  induction names generalizing Γ
-
-  case nil =>
-    rw [Env.names_empty_nil heq]
-    exact Typing.one Typing.mix₀
-
-  case cons z zs ih =>
-    simp [buildDisp]
-    have hzΓ: z ∈ Γ.names := by simp_all
-    obtain ⟨A, Γ', hP, hServ', hNames'⟩ := Env.extract_exp hzΓ hServ hNodupΓ
-    obtain ⟨hlcB, hlcΓ'⟩ := (Env.lc_cons.mp ((Env.lc_perm hP).mp hlc))
-    have hPMap : (Γ.map Prod.fst).Perm (z :: (Γ'.map Prod.fst)) := List.Perm.map _ hP
-    have hNodupCons : (z :: (Γ'.map Prod.fst)).Nodup := (List.Perm.nodup_iff hPMap).mp hNodupΓ
-    have hNodupΓ' : Env.Nodup Γ' := (List.nodup_cons.mp hNodupCons).2
-    apply Typing.exchange_hyper (𝒢 := [z ∶ ??A :: x ∶ 1 :: Γ'])
-    · apply Typing.w
-      · simp_all
-        have : x ≠ z := (hxΓ.1)
-        exact this.symm
-      · exact hlcB
-      · apply ih
-        · exact hServ'
-        · simp at hNodup
-          exact hNodup.2
-        · rw [heq] at hNames'
-          rw [← Finset.erase_eq] at hNames'
-          simp_all
-        · simp_all
-        · exact hlcΓ'
-        · exact hNodupΓ'
-    · apply HyperEnv.Perm.cons
-      · simp [HasPerm.perm]
-        apply List.Perm.trans
-        · apply List.Perm.swap
-        · apply List.Perm.cons
-          exact hP.symm
-      · simp
-
-@[simp] lemma Env.serverUsable_nil :
-  ?ₑ[] := by simp [Env.serverUsable]
-
-@[simp] lemma Channel.open_bound_zero {x : FPName} :
-  ($0)⸨#x⸩ = (#x) := by simp [HasOpen.open_, Channel.open]
-
-@[simp] lemma Channel.f_bound {i : Nat} :
-  (Channel.bound i).f = ∅ := by simp [Channel.f]
-
-@[simp] lemma Channel.close_free_self {x : FPName} :
-  (#x)⟪x⟫ = (.bound 0) := by simp [HasClose.close_, Channel.close]
-
-@[simp] lemma Channel.close_free_other {x y : FPName} (hneq : x ≠ y) :
-  (#y)⟪x⟫ = (#y) := by simp_all [HasClose.close_, Channel.close]
-
-@[simp] lemma Channel.close_self_bound {x : FPName} {i : Nat} :
-  (Channel.bound i)⟪x⟫ = (.bound i) := by simp [HasClose.close_, Channel.close]
-
-lemma Channel.close_not_mem {u : Channel} {z : FPName} {k : Nat} (h : z ∉ u.f) :
-  u⟪k | z⟫ = u := by
-  cases u <;> simp [HasClose.close_, Channel.close, Channel.f] at *
-  case free f => apply h
-
-lemma Proc.close_not_mem {P : Proc} {z : FPName} {k : Nat} (h : z ∉ P.f) :
-  P⟪k | z⟫ = P := by
-  induction P generalizing k <;> (
-    simp only [Proc.f, Finset.mem_union, not_or] at h
-    try simp
-  )
-  case one ih | bot ih | tensor ih | parr ih | selectL ih | selectR ih | output ih | input ih
-  | server ih | consume ih | dispose ih | duplicate ih => exact ⟨Channel.close_not_mem h.1, ih h.2⟩
-  case cut ih => exact ih h
-  case par ihP ihQ => exact ⟨ihP h.1, ihQ h.2⟩
-  case amp ihP ihQ => exact ⟨Channel.close_not_mem h.1.1, ihP h.1.2, ihQ h.2⟩
-  case link => exact ⟨Channel.close_not_mem h.1, Channel.close_not_mem h.2⟩
-
-lemma Proc.closeAll_not_mem {P : Proc} {L : List FPName} {k : Nat}
-  (h : P.f = ∅) : closeAll P k L = P := by
-  induction L generalizing k P
-  case nil => unfold closeAll ; simp
-  case cons x Γ ih =>
-    unfold closeAll
-    rw [Proc.close_not_mem]
-    · exact ih h
-    · rw [h] ; simp
-
-@[simp] lemma Channel.f_close {u : Channel} {x : FPName} {k : Nat} :
-  (u⟪k | x⟫).f = u.f \ {x} := by
-  cases u <;> simp [HasClose.close_, Channel.close, Channel.f]
-  case free f =>
-    split_ifs with heq
-    case pos => subst heq ; simp
-    case neg =>
-      ext y
-      simp_all [← ne_eq]
-      intro h
-      subst h
-      exact heq.symm
-
-@[simp] lemma Proc.f_close {P : Proc} {x : FPName} {k : Nat} :
-  (P⟪k | x⟫).f = P.f \ {x} := by
-  induction P generalizing k <;>
-    simp_all [← Finset.erase_eq, Finset.erase_union_distrib]
-
-lemma Channel.lc_le_any {u : Channel} {k i : Nat} (hle : i ≤ k) :
-  u.lc i → u.lc k := by
-  induction u
-  case free => simp [Channel.lc]
-  case bound => grind [Channel.lc]
-
-lemma Proc.lc_le_any {P : Proc} {k n i : Nat} (hle : i ≤ k) :
-  P.lc i n → P.lc k n := by
-  induction P generalizing n k i
-
-  case nil => simp [Proc.lc]
-
-  case one ih | bot ih | selectL ih | selectR ih | input ih | server ih | consume ih
-    | dispose ih =>
-    simp [Proc.lc]
-    intro hChan hProc
-    constructor
-    · exact Channel.lc_le_any hle hChan
-    · exact ih hle hProc
-
-  case tensor ih | parr ih | duplicate ih =>
-    simp [Proc.lc]
-    intro hChan hProc
-    constructor
-    · exact Channel.lc_le_any hle hChan
-    · exact ih (by simp [hle]) hProc
-
-  case cut ih =>
-    simp [Proc.lc] at ⊢ ih
-    intro hProc
-    apply ih (by simp [hle]) hProc
-
-  case par ihP ihQ =>
-    simp [Proc.lc]
-    intro hP hQ
-    constructor
-    · exact ihP hle hP
-    · exact ihQ hle hQ
-
-  case amp ihP ihQ =>
-    simp [Proc.lc]
-    intro hChan hP hQ
-    split_ands
-    · exact Channel.lc_le_any hle hChan
-    · exact ihP hle hP
-    · exact ihQ hle hQ
-
-  case output ih =>
-    simp [Proc.lc]
-    intro hChan hProc hlc
-    split_ands
-    · exact Channel.lc_le_any hle hChan
-    · exact ih hle hProc
-    · exact hlc
-
-  case link =>
-    simp [Proc.lc]
-    intro hx hy
-    constructor
-    · exact Channel.lc_le_any hle hx
-    · exact Channel.lc_le_any hle hy
-
-lemma Channel.lc_le {u : Channel} {k : Nat} :
-  u.lc k → u.lc (k + 1) := by
-  intro h
-  exact (Channel.lc_le_any) (by simp) h
-
-lemma Proc.lc_le {P : Proc} {k n : Nat} :
-  P.lc k n → P.lc (k + 1) n := by
-  intro h
-  exact (Proc.lc_le_any) (by simp) h
-
-@[simp] lemma Channel.lc_bound {k i : Nat} (hl : i < k) :
-  Channel.lc k (.bound i) := by simp [Channel.lc, hl]
-
-@[simp] lemma Channel.lc_close {u : Channel} {x : FPName} {k i : Nat} (hle : i ≤ k) :
-  u.lc k → u⟪i | x⟫.lc (k + 1) := by
-  induction u
-  case free y =>
-    intro h
-    simp [Channel.lc, HasClose.close_, Channel.close]
-    split_ifs
-    case pos heq => subst heq ; grind
-    case neg hneq => simp
-  case bound i =>
-    simp [Channel.lc, HasClose.close_, Channel.close]
-    grind
-
-@[simp] lemma Proc.lc_close {P : Proc} {x : FPName} {n k i : Nat} (hle : i ≤ k) :
-  P.lc k n → P⟪i | x⟫.lc (k + 1) n := by
-  induction P generalizing n k i
-
-  case nil =>
-    simp [Proc.lc]
-
-  case one ih | bot ih | selectL ih | selectR ih | input ih | server ih | consume ih
-    | dispose ih =>
-    simp [Proc.lc]
-    intro hChan hProc
-    constructor
-    · exact Channel.lc_close hle hChan
-    · apply ih hle hProc
-
-  case tensor ih | parr ih | duplicate ih =>
-    simp [Proc.lc]
-    intro hChan hProc
-    constructor
-    · exact Channel.lc_close hle hChan
-    · apply ih (by simp [hle]) hProc
-
-  case cut ih =>
-    simp [Proc.lc] at ⊢ ih
-    apply ih
-    grind
-
-  case par ihP ihQ =>
-    simp [Proc.lc] at ⊢ ihP ihQ
-    intro hP hQ
-    constructor
-    · exact ihP hle hP
-    · exact ihQ hle hQ
-
-  case amp ihP ihQ =>
-    simp [Proc.lc] at ⊢ ihP ihQ
-    intro hChan hP hQ
-    split_ands
-    · exact Channel.lc_close hle hChan
-    · exact ihP hle hP
-    · exact ihQ hle hQ
-
-  case output ih =>
-    simp [Proc.lc] at ⊢ ih
-    intro hChan hProc hType
-    split_ands
-    · exact Channel.lc_close hle hChan
-    · exact ih hle hProc
-    · exact hType
-
-  case link =>
-    simp [Proc.lc]
-    intro hx hy
-    constructor
-    · exact Channel.lc_close hle hx
-    · exact Channel.lc_close hle hy
-
-lemma Channel.close_substNames_comm_gen {u : Channel} {x y z : FPName} {k : Nat}
-  (hzx : z ≠ x) (hzy : z ≠ y) :
-  u⟪k | z⟫{y // x} = u{y // x}⟪k | z⟫ := by
-  induction u
-  case free =>
-    simp [HasClose.close_, Channel.close, HasSubst.subst, Channel.subst]
-    split_ifs
-    case pos h1 h2 => subst h1 h2 ; contradiction
-    case neg h1 h2 => simp [h1]
-    case pos h1 h2 => subst h2 ; simp [hzy]
-    case neg h1 h2 => simp ; split_ifs ; rfl
-
-  case bound =>
-    simp [HasClose.close_, Channel.close, HasSubst.subst, Channel.subst]
-
-lemma Proc.close_substNames_comm_gen {P : Proc} {x y z : FPName} {k : Nat}
-  (hzx : z ≠ x) (hzy : z ≠ y) :
-  P⟪k | z⟫{y // x} = P{y // x}⟪k | z⟫ := by
-  induction P generalizing k <;> try simp
-
-  case one ih | bot ih | tensor ih | parr ih | selectL ih | selectR ih | output ih | input ih
-    | server ih | consume ih | duplicate ih | dispose ih =>
-    exact ⟨Channel.close_substNames_comm_gen hzx hzy, ih⟩
-
-  case cut ih => exact ih
-  case par ihP ihQ => exact ⟨ihP, ihQ⟩
-  case amp ihP ihQ => exact ⟨Channel.close_substNames_comm_gen hzx hzy, ⟨ihP, ihQ⟩⟩
-  case link => simp [Channel.close_substNames_comm_gen hzx hzy]
-
-lemma Proc.close_substNames_comm {P : Proc} {x y z : FPName} (hzx : z ≠ x) (hzy : z ≠ y) :
-  P⟪z⟫{y // x} = P{y // x}⟪z⟫ := Proc.close_substNames_comm_gen (k := 0) hzx hzy
-
-lemma Proc.closeCut_substNames_comm {P : Proc} {x y z w : FPName}
-  (hzx : z ≠ x) (hzy : z ≠ y) (hwx : w ≠ x) (hwy : w ≠ y) :
-  P⟪z, w⟫{y // x} = P{y // x}⟪z, w⟫ := by
-  simp [HasCloseTwo.close_, HasSubst.subst]
-  change P⟪1 | w⟫⟪z⟫{y // x} = P{y // x}⟪1 | w⟫⟪z⟫
-  rw [Proc.close_substNames_comm_gen (k := 0) hzx hzy]
-  rw [Proc.close_substNames_comm_gen (k := 1) hwx hwy]
-
-lemma Proc.closeAll_open_substNames {P : Proc} {names : List FPName} {y z : FPName} {k n : Nat}
-  (hF : z ∉ P.f) (hlc : lc k n P) (hNodup : (names ++ [y]).Nodup) (hFz : z ∉ names) :
-  (closeAll P k (names ++ [y]))⸨k + names.length | #z⸩ = closeAll (P{z // y}) k names := by
-  induction names generalizing k P
-  case nil =>
-    simp [closeAll]
-    rw [Proc.close_open_eq_substNames]
-    · exact hF
-    · exact hlc
-
-  case cons fst names ih =>
-    simp [← ne_eq, closeAll] at ⊢ hNodup hFz
-
-    have := ih
-      (k := k + 1) (P := P⟪k | fst⟫) (by simp [hF])
-      (Proc.lc_close (by simp) hlc) hNodup.2 hFz.2
-    rw [Nat.add_assoc, Nat.add_comm 1 names.length] at this
-
-    rw [Proc.close_substNames_comm_gen] at this
-    · exact this
-    · exact hNodup.1.2
-    · apply (hFz.1).symm
-
-lemma Proc.open_wrapDup {P : Proc} {names : List FPName} {z : FPName} {k : Nat} :
-  (wrapDup P names)⸨k | #z⸩ = wrapDup (P⸨k + names.length | #z⸩) names := by
-  induction names generalizing k
-  case nil =>
-    simp [wrapDup]
-  case cons y ys ih =>
-    simp only [wrapDup, HasOpen.open_, Proc.open, List.length_cons] at ⊢ ih
-    rw [ih]
-    congr 2
-    grind
-
-lemma Env.not_mem_names_substNames {Γ : Env} {x y z : FPName} (hzy : z ≠ y) (hz : z ∉ Γ.names) :
-  z ∉ Γ{y // x}.names := by
-  induction Γ
-  case nil => simp
-  case cons E Δ ih =>
-    obtain ⟨w, T⟩ := E
-    simp at ⊢ hz
-    constructor
-    · simp [HasSubst.subst, FPName.subst]
-      split_ifs
-      case pos => exact hzy
-      case neg => exact hz.1
-    · simp_all
-
-@[simp] lemma Env.lc_nil {n : Nat} :
-  Env.lc n ([] : Env) := by simp [Env.lc]
-
-lemma Env.substNames_preserves_lc {Γ : Env} {x y : FPName} {n : Nat} (hlc : Env.lc n Γ) :
-  Env.lc n Γ{y // x} := by
-  induction Γ
-  case nil => simp
-  case cons E Δ ih =>
-    obtain ⟨w, T⟩ := E
-    simp [Env.lc_cons] at ⊢ hlc
-    constructor
-    · exact hlc.1
-    · apply ih
-      exact hlc.2
-
-lemma Env.serverUsable_perm_mp {Γ Δ : Env} :
-  Γ ~ Δ → (?ₑΓ → ?ₑΔ) := by
-  intro hP hServ A B
-  simp [Env.serverUsable] at hServ
-  have hAΓ : A ∈ Γ := (hP.mem_iff).mpr B
-  exact hServ A.1 A.2 hAΓ
-
-lemma Env.serverUsable_perm_iff {Γ Δ : Env} :
-  Γ ~ Δ → (?ₑΓ ↔ ?ₑΔ) := by
-  intro hP
-  constructor
-  · exact Env.serverUsable_perm_mp hP
-  · exact Env.serverUsable_perm_mp hP.symm
-
-lemma Env.serverUsable_merge_mp {Γ Δ : Env} :
-  ?ₑ(Γ ++ Δ) → (?ₑΓ ∧ ?ₑΔ) := by
-  simp [Env.serverUsable]
-  intro h
-  constructor
-  · intro a b hΓ
-    exact h a b (Or.inl hΓ)
-  · intro a b hΔ
-    exact h a b (Or.inr hΔ)
-
-lemma Env.serverUsable_merge_mpr {Γ Δ : Env} :
-  (?ₑΓ ∧ ?ₑΔ) → ?ₑ(Γ ++ Δ) := by
-  simp [Env.serverUsable]
-  intro hΓ hΔ a b h
-  cases h
-  case inl h => exact hΓ a b h
-  case inr h => exact hΔ a b h
-
-lemma Env.serverUsable_merge_iff {Γ Δ : Env} :
-  ?ₑ(Γ ++ Δ) ↔ (?ₑΓ ∧ ?ₑΔ) := by
-  constructor
-  · exact Env.serverUsable_merge_mp
-  · exact Env.serverUsable_merge_mpr
-
-lemma Env.Nodup_merge_iff {Γ Δ : Env} :
-  (Γ ++ Δ).Nodup ↔ (Γ.Nodup ∧ Δ.Nodup ∧ Γ.disjoint Δ) := by
-  simp [Env.Nodup]
-  constructor
-  · intro h
-    have h' := (List.nodup_append.mp h)
-    split_ands
-    · exact h'.1
-    · exact h'.2.1
-    · simp [Disjoint]
-      intro x hxΓ hxΔ
-      ext a
-      constructor
-      · intro ha
-        rcases h' with ⟨_, _, hdis⟩
-        have hΓ := hxΓ ha
-        have hΔ := hxΔ ha
-        have : a ≠ a := hdis a (by simpa using hΓ) a (by simpa using hΔ)
-        exact (this rfl).elim
-      · intro h; cases h
-  · intro h
-    obtain ⟨h1, h2, h3⟩ := h
-    have := (List.nodup_append.mpr ⟨h1, h2, ?_⟩)
-    · exact this
-    · simp [Disjoint] at h3
-      intro a ha b hb hEq
-      have hsubsetΓ : ({a} : Finset FPName) ⊆ Γ.names := by
-        intro x hx
-        simp at hx
-        subst hx
-        simpa using ha
-
-      have hsubsetΔ : ({a} : Finset FPName) ⊆ Δ.names := by
-        intro x hx
-        simp at hx
-        subst hx
-        simpa [hEq] using hb
-
-      have hEmpty := h3 hsubsetΓ hsubsetΔ
-      simp at hEmpty
-
-lemma Env.mem_unique {Γ : Env} {x : FPName} {A B : Types}
-  (hNodup : Γ.Nodup) (hA : (x, A) ∈ Γ) (hB : (x, B) ∈ Γ) : A = B := by
-  induction Γ
-  case nil => contradiction
-  case cons hd tl ih =>
-    obtain ⟨w, T⟩ := hd
-    simp_all
-    rw [Env.Nodup_cons] at hNodup
-    grind [mem_pair_fst_in_names_iff]
-
-lemma Typing_buildDup_aux {n : Nat} {QL QR : Proc} {x : FPName} {A : Types}
+lemma ProcStep_buildDup_aux {n : Nat} {QL QR : Proc} {x : FPName} {A : Types}
   (names : List FPName) (Γ Γ' ΓL : Env) (hTL : n ⊢ QL ∷ [x ∶ A :: ΓL])
   (hTR : n ⊢ QR ∷ [x ∶ A :: Γ]) (h_valid_names : ∀ z ∈ names, z ∈ Γ.names)
   (h_sync_types : ∀ z A, z ∈ names → (z, A) ∈ Γ → (z, A) ∈ ΓL)
@@ -1293,7 +287,7 @@ lemma Typing_buildDup_aux {n : Nat} {QL QR : Proc} {x : FPName} {A : Types}
       · apply List.Perm.cons
         apply List.Perm.append_right _ hP.symm
 
-lemma Typing_buildDup {n : Nat} {P : Proc} {x : FPName} {A : Types} {Γ : Env}
+lemma ProcStep_buildDup {n : Nat} {P : Proc} {x : FPName} {A : Types} {Γ : Env}
   {names : List FPName} (hServ : ?ₑΓ) (heq_names : names.toFinset = Γ.names)
   (hnd_names : names.Nodup) (hT : n ⊢ P ∷ [x ∶ A :: Γ]) :
   n ⊢ buildDup P names x ∷ [x ∶ !!A ⨂ !!A :: Γ] := by
@@ -1308,7 +302,7 @@ lemma Typing_buildDup {n : Nat} {P : Proc} {x : FPName} {A : Types} {Γ : Env}
   simp [- Env.mem_pair_fst_in_names_iff, - Env.not_mem_names_iff,
     HyperEnv.Nodup, Env.Nodup_cons, Env.lc_cons] at hndΓ hlin hlcΓx
 
-  apply Typing_buildDup_aux names Γ [] Γ
+  apply ProcStep_buildDup_aux names Γ [] Γ
   · exact hT
   · exact hT
   · intro z hz
@@ -1333,527 +327,48 @@ lemma Typing_buildDup {n : Nat} {P : Proc} {x : FPName} {A : Types} {Γ : Env}
   · exact hnd_names
   · use Γ ; simp [HasPerm.perm, heq_names]
 
+lemma ProcStep_buildDisp {n : Nat} {x : FPName} (Γ : Env) (names : List FPName)
+  (hServ : ?ₑΓ) (hNodup : names.Nodup) (heq : Γ.names = names.toFinset)
+  (hxΓ : x ∉ Γ.names) (hlc : Γ.lc n) (hNodupΓ : Env.Nodup Γ)
+  : n ⊢ buildDisp names x ∷ [x ∶ 1 :: Γ] := by
+  induction names generalizing Γ
+
+  case nil =>
+    rw [Env.names_empty_nil heq]
+    exact Typing.one Typing.mix₀
+
+  case cons z zs ih =>
+    simp [buildDisp]
+    have hzΓ: z ∈ Γ.names := by simp_all
+    obtain ⟨A, Γ', hP, hServ', hNames'⟩ := Env.extract_exp hzΓ hServ hNodupΓ
+    obtain ⟨hlcB, hlcΓ'⟩ := (Env.lc_cons.mp ((Env.lc_perm hP).mp hlc))
+    have hPMap : (Γ.map Prod.fst).Perm (z :: (Γ'.map Prod.fst)) := List.Perm.map _ hP
+    have hNodupCons : (z :: (Γ'.map Prod.fst)).Nodup := (List.Perm.nodup_iff hPMap).mp hNodupΓ
+    have hNodupΓ' : Env.Nodup Γ' := (List.nodup_cons.mp hNodupCons).2
+    apply Typing.exchange_hyper (𝒢 := [z ∶ ??A :: x ∶ 1 :: Γ'])
+    · apply Typing.w
+      · simp_all
+        have : x ≠ z := (hxΓ.1)
+        exact this.symm
+      · exact hlcB
+      · apply ih
+        · exact hServ'
+        · simp at hNodup
+          exact hNodup.2
+        · rw [heq] at hNames'
+          rw [← Finset.erase_eq] at hNames'
+          simp_all
+        · simp_all
+        · exact hlcΓ'
+        · exact hNodupΓ'
+    · apply HyperEnv.Perm.cons
+      · simp [HasPerm.perm]
+        apply List.Perm.trans
+        · apply List.Perm.swap
+        · apply List.Perm.cons
+          exact hP.symm
+      · simp
 
-
-
-lemma Typing_inv_res {n : ℕ} {P : Proc} {𝒢 : HyperEnv}
-  (hT : n ⊢ 𝑣⸨$N,$N⸩ P ∷ 𝒢) :
-  ∃ (A : Types) (Γ Δ : Env) (𝒢' : HyperEnv) (L : Finset FPName),
-    (𝒢 ~ 𝒢' |ₕ [Γ‚ Δ]) ∧
-    (∀ x ∉ L, ∀ y ∉ L, x ≠ y →
-      n ⊢ P⸨#x, #y⸩ ∷ 𝒢' |ₕ [x ∶ A :: Γ] |ₕ [y ∶ Aᗮ :: Δ]) := by
-
-  generalize heq : (𝑣⸨$N,$N⸩ P) = P' at hT
-  induction hT generalizing P <;> try contradiction
-
-  case exchange_env hP ih =>
-    obtain ⟨A, Γ, Δ, 𝒢, L, hP', hT'⟩ := ih heq
-    use A, Γ, Δ, 𝒢, L
-    constructor
-    · exact HyperEnv.Perm.trans (HyperEnv.Perm.cons hP.symm (by rfl)) hP'
-    · intros x hx y hy hneq
-      exact hT' x hx y hy hneq
-
-  case exchange_hyper hP ih =>
-    obtain ⟨A, Γ, Δ, 𝒢, L, hP', hT'⟩ := ih heq
-    use A, Γ, Δ, 𝒢, L
-    constructor
-    · exact HyperEnv.Perm.trans hP.symm hP'
-    · intros x hx y hy hneq
-      exact hT' x hx y hy hneq
-
-  case cut 𝒢 Γ Δ _ A _ L hT ih =>
-    use A, Γ, Δ, 𝒢, L
-    constructor
-    · rfl
-    · injection heq with heq
-      subst heq
-      intros x hx y hy hneq
-      exact hT x y hx hy hneq
-
-
-
-
-lemma HyperEnv.merge_nilL (𝒢 : HyperEnv) : [] |ₕ 𝒢 = 𝒢 := by simp
-
-lemma HyperEnv.merge_nilR (𝒢 : HyperEnv) : 𝒢 |ₕ [] = 𝒢 := by simp
-
-lemma HyperEnv.Perm.merge_right {𝒢 ℋ : HyperEnv} (p : 𝒢 ~ ℋ) : ∀ 𝒥, 𝒢 |ₕ 𝒥 ~ ℋ |ₕ 𝒥 := by
-  induction p
-  case nil => simp
-  case cons hPE hPH ih => intro 𝒥 ; exact HyperEnv.Perm.cons hPE (ih 𝒥)
-  case swap => intro 𝒥 ; exact HyperEnv.Perm.swap ..
-  case trans ih1 ih2 => intro 𝒥 ; exact HyperEnv.Perm.trans (ih1 𝒥) (ih2 𝒥)
-
-theorem HyperEnv.Perm.merge_left {𝒢 ℋ : HyperEnv} : 𝒢 ~ ℋ → ∀ 𝒥, 𝒥 |ₕ 𝒢 ~ 𝒥 |ₕ ℋ := by
-  intro h 𝒥
-  induction 𝒥
-  case nil => exact h
-  case cons Γ ℐ ih => apply HyperEnv.Perm.cons (.refl _) ih
-
-theorem HyperEnv.Perm.merge {𝒢 𝒢' ℋ ℋ' : HyperEnv} (p₁ : 𝒢 ~ 𝒢') (p₂ : ℋ ~ ℋ') :
-  𝒢 |ₕ ℋ ~ 𝒢' |ₕ ℋ' := (p₁.merge_right ℋ).trans (p₂.merge_left _)
-
-@[simp] lemma HyperEnv.Perm_middle {Γ : Env} : ∀ {𝒢 ℋ : HyperEnv}, 𝒢 |ₕ Γ :: ℋ ~ Γ :: (𝒢 |ₕ ℋ)
-  | [], _ => .refl _
-  | Δ :: _, _ =>
-    (HyperEnv.Perm.cons (.refl _) Perm_middle).trans (HyperEnv.Perm.swap Δ Γ _)
-
-lemma HyperEnv.Perm.merge_exchange_right {𝒢 ℋ 𝒥 : HyperEnv} :
-  ℋ ~ 𝒥 → (𝒢 |ₕ ℋ ~ 𝒢 |ₕ 𝒥) := by
-  intro h
-  induction 𝒢
-  case nil => simp ; exact h
-  case cons ih => apply HyperEnv.Perm.cons (by rfl) ih
-
-lemma HyperEnv.Perm.merge_exchange_left {𝒢 ℋ 𝒥 : HyperEnv} :
-  ℋ ~ 𝒥 → (ℋ |ₕ 𝒢 ~ 𝒥 |ₕ 𝒢 ) := by
-  intro h
-  induction h
-  case nil => simp
-  case cons hPE hPH ih => exact HyperEnv.Perm.cons hPE ih
-  case swap => exact HyperEnv.Perm.swap ..
-  case trans ih1 ih2 => exact HyperEnv.Perm.trans ih1 ih2
-
-lemma HyperEnv.Perm.merge_comm : ∀ {𝒢 ℋ : HyperEnv}, 𝒢 |ₕ ℋ ~ ℋ |ₕ 𝒢
-  | [], _ => by simp
-  | _ :: _, _ => (HyperEnv.Perm.merge_comm.cons (.refl _)).trans HyperEnv.Perm_middle.symm
-
-lemma HyperEnv.merge_assoc (𝒢 ℋ ℐ : HyperEnv) : 𝒢 |ₕ ℋ |ₕ ℐ = 𝒢 |ₕ (ℋ |ₕ ℐ) := by
-  simp only [List.append_assoc]
-
-lemma HyperEnv.Perm.merge_assoc (𝒢 ℋ ℐ : HyperEnv) :
-  (𝒢 |ₕ (ℋ |ₕ ℐ)) ~ (ℋ |ₕ (𝒢 |ₕ ℐ)) := by
-  repeat rw [← HyperEnv.merge_assoc]
-  apply HyperEnv.Perm.merge_right HyperEnv.Perm.merge_comm
-
-lemma HyperEnv.Perm.merge_cons {Γ : Env} {𝒢 𝒢' ℋ ℋ' : HyperEnv} (p₁ : 𝒢 ~ 𝒢') (p₂ : ℋ ~ ℋ') :
-    𝒢 |ₕ Γ :: ℋ ~ 𝒢' |ₕ Γ :: ℋ' := p₁.merge (p₂.cons (.refl _))
-
-@[simp] lemma HyperEnv.Perm_merge_singleton (Γ : Env) (𝒢 : HyperEnv) : 𝒢 |ₕ [Γ] ~ Γ :: 𝒢 :=
-  HyperEnv.Perm_middle.trans <| by rw [HyperEnv.merge_nilR]
-
-lemma HyperEnv.Perm_merge_comm : ∀ {𝒢 ℋ : HyperEnv}, 𝒢 |ₕ ℋ ~ ℋ |ₕ 𝒢
-  | [], _ => by simp
-  | _ :: _, _ => (HyperEnv.Perm_merge_comm.cons (.refl _)).trans HyperEnv.Perm_middle.symm
-
-theorem HyperEnv.Perm_merge_comm_assoc (𝒢 ℋ 𝒥 : HyperEnv) :
-    (𝒢 |ₕ (ℋ |ₕ 𝒥)) ~ (ℋ |ₕ (𝒢 |ₕ 𝒥)) := by
-  simpa only [List.append_assoc] using HyperEnv.Perm_merge_comm.merge_right _
-
-lemma HyperEnv.cons_rotate_left (𝒢 : HyperEnv) (Γ : Env) :
-  (Γ :: 𝒢) ~ (𝒢 |ₕ [Γ]) := by
-  symm ; apply HyperEnv.Perm_merge_singleton
-
-lemma HyperEnv.cons_append {𝒢 : HyperEnv} {Γ : Env} :
-  Γ :: 𝒢 = [Γ] |ₕ 𝒢 := by simp
-
-inductive HyperEnv.Delete (Γ : Env) : HyperEnv → HyperEnv → Prop where
-  | head {𝒢 : HyperEnv} {Δ : Env} :
-      (Γ ~ Δ) → Delete Γ (Δ :: 𝒢) 𝒢
-  | tail {Δ : Env} {𝒢 𝒢' : HyperEnv} :
-      Delete Γ 𝒢 𝒢' → Delete Γ (Δ :: 𝒢) (Δ :: 𝒢')
-
--- Removing Γ from Γ :: 𝒢 => 𝒢 then adding Γ again => Γ :: 𝒢
-lemma HyperEnv.Delete_restore {Γ : Env} {𝒢 𝒢' : HyperEnv} (h : Delete Γ 𝒢 𝒢') :
-  Γ :: 𝒢' ~ 𝒢 := by
-  induction h
-  case head Δ hEnv =>
-    exact HyperEnv.Perm.cons hEnv (.refl _)
-  case tail Δ hD ih =>
-    apply HyperEnv.Perm.trans (HyperEnv.Perm.swap ..)
-    exact HyperEnv.Perm.cons (List.Perm.refl _) ih
-
-lemma HyperEnv.Perm_Delete {𝒢 ℋ : HyperEnv} (hP : 𝒢 ~ ℋ) :
-  ∀ {Γ 𝒢'}, Delete Γ 𝒢 𝒢' → ∃ ℋ', Delete Γ ℋ ℋ' ∧ 𝒢' ~ ℋ' := by
-  induction hP
-  case nil => intros _ 𝒢 _ ; use 𝒢
-
-  case cons Γ Δ 𝒢 ℋ hPE hPH ih =>
-    intros Ξ 𝒥 hDel
-    cases hDel
-    case head hP' =>
-      exact ⟨ℋ, HyperEnv.Delete.head (List.Perm.trans hP' hPE), hPH⟩
-    case tail 𝒥 hDel =>
-      obtain ⟨ℋ', hDelℋ', hPℋ'⟩ := ih hDel
-      exact ⟨Δ :: ℋ', HyperEnv.Delete.tail hDelℋ', HyperEnv.Perm.cons hPE hPℋ'⟩
-
-  case swap Γ Δ 𝒢 =>
-    intro Ξ 𝒢' hDel
-    cases hDel
-    case head hEnv =>
-      exact ⟨Δ :: 𝒢, HyperEnv.Delete.tail (HyperEnv.Delete.head hEnv), .refl _⟩
-    case tail hD_tail =>
-      cases hD_tail
-      case head hPE =>
-        use Γ :: 𝒢
-        exact ⟨HyperEnv.Delete.head hPE, .refl _⟩
-      case tail 𝒢' hD_tl_tl =>
-        exact ⟨Δ :: Γ :: 𝒢', HyperEnv.Delete.tail (HyperEnv.Delete.tail hD_tl_tl), .swap ..⟩
-
-  case trans ih1 ih2 =>
-    intros E1 H1 hDel1
-    obtain ⟨H2, hDel2, hP12⟩ := ih1 hDel1
-    obtain ⟨H3, hDel3, hP23⟩ := ih2 hDel2
-    exact ⟨H3, hDel3, HyperEnv.Perm.trans hP12 hP23⟩
-
-lemma HyperEnv.Perm.cons_cancel_left {Γ : Env} {𝒢 ℋ : HyperEnv} (hP : Γ :: 𝒢 ~ Γ :: ℋ) :
-  𝒢 ~ ℋ := by
-  have hDel1 : Delete Γ (Γ :: 𝒢) 𝒢 := Delete.head (List.Perm.refl _)
-  obtain ⟨_, hDel2, hP'⟩ := HyperEnv.Perm_Delete hP hDel1
-  cases hDel2
-  case head _ => exact hP'
-  case tail hDel3 =>
-    apply HyperEnv.Perm.trans hP'
-    exact HyperEnv.Delete_restore hDel3
-
-lemma HyperEnv.Perm_merge_cancel_right {𝒢 ℋ 𝒥 : HyperEnv} :
-  𝒢 |ₕ 𝒥 ~ ℋ |ₕ 𝒥 → 𝒢 ~ ℋ := by
-  intro h
-  induction 𝒥 generalizing 𝒢 ℋ
-  case nil => simp at h ; exact h
-  case cons Γ 𝒥 ih =>
-    rw [HyperEnv.cons_append, ← HyperEnv.merge_assoc, ← HyperEnv.merge_assoc] at h
-    have hcancel := (ih h)
-    have h_front : Γ :: 𝒢 ~ Γ :: ℋ := by
-      apply HyperEnv.Perm.trans (HyperEnv.Perm_merge_singleton Γ 𝒢).symm
-      apply HyperEnv.Perm.trans hcancel
-      exact HyperEnv.Perm_merge_singleton Γ ℋ
-    exact HyperEnv.Perm.cons_cancel_left h_front
-
-lemma HyperEnv.Perm_merge_cancel_left {𝒢 ℋ 𝒥 : HyperEnv} :
-  𝒥 |ₕ 𝒢 ~ 𝒥 |ₕ ℋ → 𝒢 ~ ℋ := by
-  intro h
-  induction 𝒥
-  case nil => exact h
-  case cons Ξ 𝒥' ih => exact ih (HyperEnv.Perm.cons_cancel_left h)
-
-
-
-
--- FIXME: Fix TypingStep
--- FIXME: Typing_preserves_proc_congr
--- FIXME: Use NameSpaces instead of having e.g. HyperEnv._____ everywhere
-
-
-
-
--- FIXME: Proof showing substitution avoids capture
--- FIXME: Proof showing AlphaEq is equivalent to = between Procs
--- FIXME: Find different syntax for open?
--- FIXME: Prove name substitution only being applied to free names?
-
-
--- NOTE: shows the proof lean found using the simp_all tactic show_term { simp_all }
-
--- TODO: Implement the following instead of having post condition on res in EnvStep
--- NOTE: Not possible without knowning that l.i is disjoint form ℋ, which could be
--- obtained from a ProcStep sidecondition, but that would require having this be used
--- inside e.g. session_fidelity and not having it be a strictly stand alone property /
--- lemma for EnvStep - This would also need to know the corresponding ProcStep and Typing.
--- But could work as an auxiliary for session fidelity, not standalone for EnvStep.
--- lemma EnvStep.Linearity_and_subset {𝒢 𝒢' : HyperEnv} {l : Lbl}
---   (hlin : 𝒢.Linearity) (hES : 𝒢 -[l]->ₑ 𝒢') :
---   𝒢'.Linearity ∧ (𝒢'.names ⊆ 𝒢.names ∪ l.i) := by
---   induction hES
-
-
-
-
--- FIXME: Currently HyperEnv.Nodup is only internal for each parallel componenet
---        and PairwiseDisjoint checks intra disjointess for components.
---        Change this to have global no duplicates predicate using current Nodup
---        and PairwiseDisjoint.
-
--- FIXME: Move everything related to HyperEnv.Perm to a separate file?
-
-
-lemma HyperEnv.disjoint_names_left {𝒢 : HyperEnv} {S : Finset FPName} :
-  Disjoint 𝒢.names S ↔ ∀ Γ ∈ 𝒢, Disjoint Γ.names S := by
-  induction 𝒢
-  case nil => simp
-  case cons ih =>
-    simp [HyperEnv.names_cons]
-    intro
-    apply ih
-
-lemma HyperEnv.disjoint_names_right {𝒢 : HyperEnv} {S : Finset FPName} :
-  Disjoint S 𝒢.names ↔ ∀ Γ ∈ 𝒢, Disjoint S Γ.names := by
-  induction 𝒢
-  case nil => simp
-  case cons ih =>
-    simp [HyperEnv.names_cons]
-    intro
-    apply ih
-
-def HyperEnv.Linearity (𝒢 : HyperEnv) : Prop :=
-  𝒢.Nodup ∧ 𝒢.PairwiseDisjoint
-
-lemma HyperEnv.Perm_preserves_Linearity {𝒢 ℋ : HyperEnv} :
-  𝒢 ~ ℋ → (𝒢.Linearity ↔ ℋ.Linearity) := by
-  intro h
-  simp [HyperEnv.Linearity, HyperEnv.PairwiseDisjoint]
-  rw [HyperEnv.Nodup_perm_iff h, HyperEnv.Perm_PairwiseDisjoint_iff h]
-
-lemma HyperEnv.Perm.preserves_Linearity {𝒢 ℋ : HyperEnv}
-  (hP : 𝒢 ~ ℋ) (h : 𝒢.Linearity) : ℋ.Linearity :=
-  (HyperEnv.Perm_preserves_Linearity hP).mp h
-
-@[simp] lemma HyperEnv.Linearity_nil :
-  HyperEnv.Linearity [] := by simp [HyperEnv.Linearity]
-
-@[simp] lemma HyperEnv.Linearity_singleton {Γ : Env} :
-  HyperEnv.Linearity [Γ] = Γ.Nodup := by
-  simp [HyperEnv.Linearity, HyperEnv.Nodup]
-
-@[simp] lemma HyperEnv.Linearity_merge {𝒢 ℋ : HyperEnv} :
-  (𝒢 |ₕ ℋ).Linearity = (𝒢.Linearity ∧ ℋ.Linearity ∧
-    ∀ a ∈ 𝒢, ∀ b ∈ ℋ, Disjoint a.names b.names) := by
-  simp [HyperEnv.Linearity]
-  constructor
-  · intro h
-    obtain ⟨⟨h1, h2⟩, h3, h4, h5⟩ := h
-    exact ⟨⟨h1, h3⟩, ⟨⟨h2, h4⟩, h5⟩⟩
-  · intro h
-    obtain ⟨⟨h1, h2⟩, ⟨h3, h4⟩, h5⟩ := h
-    exact ⟨⟨h1, h3⟩, h2, h4, h5⟩
-
--- NOTE: There have been placed additional constraints on par₁, par₂, res and syn in EnvStep to
--- make this a standalone property, and getting it to type check. Ideally, these would be removed
--- and mutual induction would be done on ProcStep and EnvStep related by a valid Typing instead.
--- The added contraints are either provided by constraints on ProcStep or can be extracted from
--- The Typing relation using the `Typing_preserves_XXX` lemmas.
-lemma EnvStep.preserves_Linearity {𝒢 𝒢' : HyperEnv} {l : Lbl}
-  (hlin : 𝒢.Linearity) (hES : 𝒢 -[l]->ₑ 𝒢') : 𝒢'.Linearity := by
-  induction hES
-
-  case one | link₁ => simp
-
-  case tensor hF =>
-    simp [HyperEnv.Linearity, HyperEnv.Nodup, Env.Nodup_cons, Env.Nodup_merge_iff] at ⊢ hlin hF
-    split_ands
-    · exact hF.2.1
-    · exact hlin.2.1
-    · exact hlin.1.2
-    · exact hlin.2.2.1
-    · simp_all [← ne_eq, HyperEnv.PairwiseDisjoint]
-      exact hF.1.symm
-
-  case bot =>
-    simp [HyperEnv.Linearity, HyperEnv.Nodup, Env.Nodup_cons] at ⊢ hlin
-    exact hlin.2
-
-  case parr hF =>
-    simp [HyperEnv.Linearity, HyperEnv.Nodup, Env.Nodup_cons] at ⊢ hlin hF
-    constructor
-    · exact hF
-    · exact hlin
-
-  case par₁ hES hDl ih =>
-    simp at ⊢ hlin
-    obtain ⟨hlin𝒢, hlinℋ, hD⟩ := hlin
-    constructor
-    · exact ih hlin𝒢
-    · constructor
-      · exact hlinℋ
-      · intro E1 hE1 E2 hE2
-        have hsub𝒢'𝒢:= EnvStep.names_subset hES
-        have hsubE1 :=
-          Finset.Subset.trans (HyperEnv.subset_names_of_mem hE1) hsub𝒢'𝒢
-        apply Finset.disjoint_of_subset_left hsubE1
-        rw [Finset.disjoint_union_left]
-        constructor
-        · rw [HyperEnv.disjoint_names_left]
-          intro a ha
-          exact hD a ha E2 hE2
-        · rw [← Finset.disjoint_iff_inter_eq_empty] at hDl
-          exact Finset.disjoint_of_subset_right (HyperEnv.subset_names_of_mem hE2) hDl
-
-  case par₂ hES hDl ih =>
-    simp at ⊢ hlin
-    obtain ⟨hlin𝒢, hlinℋ, hD⟩ := hlin
-    constructor
-    · exact hlin𝒢
-    · constructor
-      · exact ih hlinℋ
-      · intro E1 hE1 E2 hE2
-        have hsubℋ'ℋ := EnvStep.names_subset hES
-        have hsubE2 :=
-          Finset.Subset.trans (HyperEnv.subset_names_of_mem hE2) hsubℋ'ℋ
-        apply Finset.disjoint_of_subset_right hsubE2
-        rw [Finset.disjoint_union_right]
-        constructor
-        · rw [HyperEnv.disjoint_names_right]
-          intro a ha
-          exact hD E1 hE1 a ha
-        · rw [← Finset.disjoint_iff_inter_eq_empty] at hDl
-          exact Finset.disjoint_of_subset_left (HyperEnv.subset_names_of_mem hE1) hDl.symm
-
-  case syn hES𝒢 hESℋ hDl lwf ihP ihQ =>
-    simp at ⊢ hlin
-    obtain ⟨hlin𝒢, hlinℋ, hD⟩ := hlin
-
-    constructor
-    · exact ihP hlin𝒢
-    · constructor
-      · exact ihQ hlinℋ
-      · intro E1 hE1 E2 hE2
-        rw [← Finset.disjoint_iff_inter_eq_empty] at hDl
-        rw [Lbl.WF, ← Finset.disjoint_iff_inter_eq_empty] at lwf
-        simp only [HyperEnv.merge, HyperEnv.names_merge, Lbl.i,
-          Finset.disjoint_union_left, Finset.disjoint_union_right] at hDl
-        obtain ⟨⟨hDl1, hDl2⟩, ⟨hDl3, hDl4⟩⟩ := hDl
-
-        have hsubE1 := Finset.Subset.trans
-          (HyperEnv.subset_names_of_mem hE1)
-          (EnvStep.names_subset hES𝒢)
-
-        have hsubE2:= Finset.Subset.trans
-          (HyperEnv.subset_names_of_mem hE2)
-          (EnvStep.names_subset hESℋ)
-
-        apply Finset.disjoint_of_subset_left hsubE1
-        apply Finset.disjoint_of_subset_right hsubE2
-
-        rw [Finset.disjoint_union_left, Lbl.i, Lbl.i]
-        constructor
-        · rw [Finset.disjoint_union_right]
-          constructor
-          · rw [HyperEnv.disjoint_names_left]
-            intro E3 hE3
-            rw [HyperEnv.disjoint_names_right]
-            intro E4 hE4
-            exact hD E3 hE3 E4 hE4
-          · exact hDl2.symm
-        · rw [Finset.disjoint_union_right]
-          constructor
-          · exact hDl3
-          · exact lwf
-
-  case one_bot | tensor_parr => exact hlin
-
-  case res 𝒢 𝒢' Γ Γ' Δ Δ' x y A B l hFx hFy hFx' hFy' _ _ hneq hES𝒢 ih =>
-    simp [Env.Nodup_merge_iff] at hlin ⊢ hFx hFx' hFy hFy'
-    obtain ⟨hlin𝒢, ⟨hndΓ, ⟨hndΔ, hDΓΔ⟩⟩, hD⟩ := hlin
-    have hlin_inner : (𝒢 |ₕ [x ∶ Aᗮ :: Γ] |ₕ [y ∶ A :: Δ]).Linearity := by
-      simp
-      constructor
-      · exact hlin𝒢
-      · constructor
-        · change HyperEnv.Linearity ([x ∶ Aᗮ :: Γ] |ₕ  [y ∶ A :: Δ])
-          simp only [HyperEnv.Linearity_merge]
-          constructor
-          · simp [Env.Nodup_cons]
-            constructor
-            · exact hFx.2.1
-            · exact hndΓ
-          · constructor
-            · simp [Env.Nodup_cons]
-              constructor
-              · exact hFy.2.2
-              · exact hndΔ
-            · intro a ha b hb
-              simp at ha hb
-              simp [ha, hb]
-              exact ⟨⟨hneq.symm, hFy.2.1⟩, ⟨hFx.2.2, hDΓΔ⟩⟩
-        · intro a ha
-          obtain ⟨hDΓ, hDΔ⟩ := hD a ha
-          refine ⟨⟨?_, hDΓ⟩, ⟨?_, hDΔ⟩⟩
-          · intro T hxT
-            apply hFx.1
-            rw [HyperEnv.mem_pair_fst_in_names]
-            use T, a
-          · intro T hyT
-            apply hFy.1
-            rw [HyperEnv.mem_pair_fst_in_names]
-            use T, a
-
-    have hlin_outer:= ih hlin_inner
-
-    simp at hlin_outer
-    obtain ⟨hlin𝒢', hlin_xy, hD'⟩ := hlin_outer
-    change HyperEnv.Linearity ([x ∶ Aᗮ :: Γ'] |ₕ  [y ∶ A :: Δ']) at hlin_xy
-    simp only [HyperEnv.Linearity_merge, HyperEnv.Linearity_singleton, Env.Nodup_cons] at hlin_xy
-    obtain ⟨hlin_xΓ', hlin_yΔ', hD_xΓ'yΔ'⟩ := hlin_xy
-    simp at hD_xΓ'yΔ'
-
-    split_ands
-    · exact hlin𝒢'.1
-    · exact hlin𝒢'.2
-    · exact hlin_xΓ'.2
-    · exact hlin_yΔ'.2
-    · exact hD_xΓ'yΔ'.2.2
-    · intro a ha
-      have ⟨⟨_, haΓ'⟩, _, haΔ'⟩:= hD' a ha
-      constructor
-      · exact haΓ'
-      · exact haΔ'
-
-  case selectL | selectR | ampL | ampR | use₁ | use₂ | disp₁ | disp₂
-    | dup₁ | dup₂ | output | input =>
-    simp [Env.Nodup_cons] at hlin ⊢
-    exact hlin
-
-  case perm hP _ hP' ih =>
-    exact hP'.preserves_Linearity (ih (hP.symm.preserves_Linearity hlin))
-
-
-
-
-
-
-
-
-
-
-
-
-lemma HyperEnv.Perm_rotate_rhs_right {𝒢 ℋ 𝒥 𝒦 : HyperEnv} :
-  𝒢 ~ ℋ |ₕ 𝒥 |ₕ 𝒦 → 𝒢 ~ 𝒥 |ₕ 𝒦 |ₕ ℋ := by
-  intro h
-  apply HyperEnv.Perm.trans
-  · exact h
-  · apply HyperEnv.Perm.trans
-    · simp only [HyperEnv.merge_assoc]
-      apply HyperEnv.Perm.merge_assoc
-    · simp only [HyperEnv.merge_assoc]
-      apply HyperEnv.Perm.merge_left
-      exact HyperEnv.Perm.merge_comm
-
-lemma HyperEnv.Perm_rotate_rhs_left {𝒢 ℋ 𝒥 𝒦 : HyperEnv} :
-  𝒢 ~ ℋ |ₕ 𝒥 |ₕ 𝒦 → 𝒢 ~ 𝒦 |ₕ ℋ |ₕ 𝒥 := by
-  intro h
-  apply HyperEnv.Perm_rotate_rhs_right
-  exact HyperEnv.Perm_rotate_rhs_right h
-
-lemma HyperEnv.Perm_pull_rhs_mid_left {𝒢 ℋ 𝒥 𝒦 : HyperEnv} :
-  𝒢 ~ ℋ |ₕ (𝒥 |ₕ 𝒦) → 𝒢 ~ 𝒥 |ₕ (ℋ |ₕ 𝒦) := by
-  intro h
-  apply HyperEnv.Perm.trans
-  · exact h
-  · apply HyperEnv.Perm.merge_assoc
-
-lemma HyperEnv.Perm_pull_rhs_mid_right {𝒢 ℋ 𝒥 𝒦 : HyperEnv} :
-  𝒢 ~ (ℋ |ₕ 𝒥) |ₕ 𝒦 → 𝒢 ~ (ℋ |ₕ 𝒦) |ₕ 𝒥 := by
-  intro h
-  apply HyperEnv.Perm.trans
-  · exact h
-  · apply HyperEnv.Perm.symm
-    conv_rhs => rw [HyperEnv.merge_assoc]
-    apply HyperEnv.Perm_pull_rhs_mid_left
-    conv_rhs => rw [← HyperEnv.merge_assoc]
-    apply HyperEnv.Perm_rotate_rhs_left
-    rfl
-
-lemma HyperEnv.Perm.exchange_lhs_left {𝒢 ℋ 𝒥 𝒦 : HyperEnv} :
-  ℋ ~ 𝒥 → ℋ |ₕ 𝒦 ~ 𝒢 → 𝒥 |ₕ 𝒦 ~ 𝒢 := by
-  intros h1 h2
-  exact (h2.symm.trans (HyperEnv.Perm.merge_right h1 _)).symm
-
-lemma HyperEnv.Perm.exchange_rhs_left {𝒢 ℋ 𝒥 𝒦 : HyperEnv} :
-  ℋ ~ 𝒥 → 𝒢 ~ ℋ |ₕ 𝒦 → 𝒢 ~ 𝒥 |ₕ 𝒦 := by
-  intros h1 h2
-  exact (h2.trans (HyperEnv.Perm.merge_right h1 _))
 
 
 
@@ -2252,7 +767,7 @@ theorem session_fidelity {n : Nat} {P P' : Proc} {𝒢 : HyperEnv} {l : Lbl} :
         have := (Env.lc_cons.mp hlcAΓ).2
         exact this
 
-      exact Typing_buildDisp Γ _ hServ hNodup_names heq hxΓ hlc hNodupΓ
+      exact ProcStep_buildDisp Γ _ hServ hNodup_names heq hxΓ hlc hNodupΓ
 
   case dup₁ x =>
     obtain ⟨Γ, A, L, hP', hF, hT'⟩ := Typing_inv_dup₁ hT
@@ -2271,7 +786,7 @@ theorem session_fidelity {n : Nat} {P P' : Proc} {𝒢 : HyperEnv} {l : Lbl} :
     use [z ∶ !!A ⨂ !!A :: Γ]
     · constructor
       · exact EnvStep.perm hP'.symm (EnvStep.dup₂ hServ) (by rfl)
-      · apply Typing_buildDup (names := (Q.f.erase z).toList)
+      · apply ProcStep_buildDup (names := (Q.f.erase z).toList)
         · exact hServ
         · simp
           rw [Typing.f_eq_names hT']
@@ -2360,6 +875,24 @@ theorem session_fidelity {n : Nat} {P P' : Proc} {𝒢 : HyperEnv} {l : Lbl} :
 
   case com => sorry
   case axcut => sorry
+
+
+
+
+lemma Env.exists_perm_cons {Γ : Env} {x : FPName} {A : Types} (h : (x, A) ∈ Γ) :
+  ∃ Δ, Γ ~ (x, A) :: Δ := by
+  induction Γ
+  case nil => simp at h
+  case cons e Ξ ih =>
+    simp at h
+    cases h
+    case inl h => subst h ; use Ξ
+    case inr h =>
+      obtain ⟨y, T⟩ := e
+      obtain ⟨Ξ', hP⟩ := ih h
+      use (y ∶ T :: Ξ)
+      sorry
+
 
 
 
@@ -2461,8 +994,8 @@ lemma HyperEnv.Perm.extract_bot_res
             · injection heq with heq_name _
               exact hneq heq_name.symm
             · exact hyΓ (Env.mem_pair_fst_in_names _ hyinΓ)
-        ·
-          have hPΔΔ' : Δ ~ Δ' := by
+
+        · have hPΔΔ' : Δ ~ Δ' := by
             simp [HasPerm.perm] at hPEy
             exact hPEy
 
@@ -2488,8 +1021,6 @@ lemma HyperEnv.Perm.extract_bot_res
           have hxinEx : x ∈ Ex.names := by
             exact Env.mem_pair_fst_in_names _ hxA
 
-
-
           simp only [List.mem_append, List.mem_singleton] at hEx_RHS
           rcases hEx_RHS with h1 | hEx_Xi | rfl
           · cases h1 with
@@ -2512,8 +1043,7 @@ lemma HyperEnv.Perm.extract_bot_res
               simp
               exact Or.inr hxA
 
-          ·
-            have hPΓΓ' : Γ ~ Γ' := by
+          · have hPΓΓ' : Γ ~ Γ' := by
               simp [HasPerm.perm] at hPEx
               exact hPEx
 
@@ -2526,19 +1056,52 @@ lemma HyperEnv.Perm.extract_bot_res
                 apply hPEx
               · rfl
 
-            have h_core : ℋ ~ 𝒢ᵣ' |ₕ [Ξ] :=
-                HyperEnv.Perm_merge_cancel_right (h_post''.trans h_post_no_y.symm)
+            rw [HyperEnv.merge_assoc]
+            apply HyperEnv.Perm_pull_rhs_mid_left
+            rw [← HyperEnv.merge_assoc]
+            apply HyperEnv.Perm_rotate_rhs_left
+            apply HyperEnv.Perm.merge
+            · exact HyperEnv.Perm_merge_cancel_right (h_post''.trans h_post_no_y.symm)
+            · symm
+              apply HyperEnv.Perm.cons
+              · exact (List.Perm.append_right Δ hPΓΓ').trans
+                  (List.Perm.append_left Γ' hPΔΔ')
+              · rfl
 
-            have h1 : [Γ'‚ Δ'] ~ [Γ‚ Δ] := by sorry
-            have h2 : ℋ |ₕ [Γ'‚ Δ'] ~ 𝒢ᵣ' |ₕ [Ξ] |ₕ [Γ'‚ Δ'] := by sorry
-            have h3 : (𝒢ᵣ' |ₕ [Ξ]) |ₕ [Γ'‚ Δ'] ~ 𝒢ᵣ' |ₕ [Ξ] |ₕ [Γ‚ Δ] := by sorry
-            have h4 : 𝒢ᵣ' |ₕ [Ξ] |ₕ [Γ‚ Δ] ~ 𝒢ᵣ' |ₕ [Γ‚ Δ] |ₕ [Ξ] := by sorry
+    · subst hEΓx
 
-            exact h2.trans (h3.trans h4)
+      have hzinΓx : (z, ⊥) ∈ x ∶ Aᗮ :: Γ := by
+        simp [HasPerm.perm] at hPE
+        have h := hPE.symm.subset
+        simp at h
+        obtain ⟨hL, hR⟩ := h
+        cases hL
+        case inl hL1 =>
+          rw [hL1.1, hL1.2]
+          simp
+        case inr hL2 =>
+          exact List.mem_cons.mpr (Or.inr hL2)
+
+
+      simp at hzinΓx
+      rcases hzinΓx with ⟨hzx, _⟩ | hin
+      · subst hzx
+        contradiction
+      ·
+        obtain ⟨Γ_rest, hΓ_split⟩ :=
+
+
+
+
+        sorry
 
 
 
 
 
-    · sorry
+
+
+
+
+      sorry
   · sorry
