PiLL/PiLL/Framework/Model/Judgement.lean
@@ -225,8 +225,7 @@ lemma Typing_preserves_lc_context {𝒢 : HyperEnv} {P : Proc} {n : Nat} :
     cases hE𝒢 <;> simp_all
 
   case one | bot | quest | bang | amp | oplus₁ | oplus₂ | w | ax =>
-    simp_all [Env.lc_cons, Types.lc_dual.mp]
-    simp_all [Env.lc, Types.lc]
+    simp_all [Env.lc_cons, Types.lc, Types.lc_dual.mp]
 
   case exists_ Γ _ x A B n hlc _ ih =>
     simp at hE𝒢
@@ -556,3 +555,493 @@ lemma Typing_preserves_linearity {n : Nat} {P : Proc} {𝒢 : HyperEnv} :
     constructor
     · exact HyperEnv.Nodup_perm hP ih1
     · exact (HyperEnv.Perm_PairwiseDisjoint_iff hP).mp ih2
+
+lemma Typing.f_eq_names {n : Nat} {P : Proc} {𝒢 : HyperEnv} :
+  (n ⊢ P ∷ 𝒢) → P.f = 𝒢.names := by
+  intro h
+  induction h <;> try simp [Channel.f]
+
+  case mix ih1 ih2 => rw [ih1, ih2]
+
+  case one ih | bot ih | oplus₁ ih | oplus₂ ih | quest ih | bang ih | w ih | exists_ ih
+    | forall_ ih =>
+    simp [ih]
+
+  case cut ℋ Γ Δ P _ _ L _ ih =>
+    have ⟨x, y, hx, hy, hneq⟩ := exists_two_fresh (L ∪ P.f ∪ ℋ.names ∪ Γ.names ∪ Δ.names)
+    simp at hx hy ih
+    obtain ⟨hx1, hx2, hx3⟩ := hx
+    obtain ⟨hy1, hy2, hy3⟩ := hy
+    have := ih x y hx1 hy1 hneq
+    apply_fun (fun s => (s.erase y).erase x) at this
+    rw [Finset.erase_insert (by simp [hy3, hneq.symm]), Finset.erase_insert (by simp [hx3]),
+      Finset.erase_right_comm, Proc.f_open_two_erase hx2 hy2 hneq] at this
+    exact this
+
+  case tensor Γ Δ P x _ _ _ _ L _ ih =>
+    obtain ⟨y, hy⟩ := exists_one_fresh (L ∪ P.f ∪ {x} ∪ Γ.names ∪ Δ.names)
+    simp at hy ih
+    obtain ⟨hneq, hy1, hy2, hy3⟩ := hy
+    have := ih y hy1
+    apply_fun (fun s => s.erase y) at this
+    rw [Proc.f_open_erase hy2, Finset.insert_comm,
+      Finset.erase_insert (by simp [hneq, hy3])] at this
+    simp [this]
+
+  case parr Γ P x _ _ _ _ L _ ih =>
+    obtain ⟨y, hy⟩ := exists_one_fresh (L ∪ P.f ∪ {x} ∪ Γ.names)
+    simp at hy ih
+    obtain ⟨hneq, hy1, hy2, hy3⟩ := hy
+    have := ih y hy1
+    apply_fun (fun s => s.erase y) at this
+    rw [Proc.f_open_erase hy2, Finset.insert_comm,
+      Finset.erase_insert (by simp [hneq, hy3])] at this
+    simp [this]
+
+  case c Γ P x _ _ _ L _ ih =>
+    obtain ⟨y, hy⟩ := exists_one_fresh (L ∪ P.f ∪ {x} ∪ Γ.names)
+    simp at hy ih
+    obtain ⟨hneq, hy1, hy2, hy3⟩ := hy
+    have := ih y hy1
+    apply_fun (fun s => s.erase y) at this
+    rw [Proc.f_open_erase hy2, Finset.erase_insert (by simp [hneq, hy3])] at this
+    simp [this]
+
+  case amp ihP ihQ => simp [ihP, ihQ]
+
+  case exchange_env hP ih =>
+    simp [ih, Env.names_eq_of_perm hP]
+
+  case exchange_hyper hP ih =>
+    simp [ih, HyperEnv.names_eq_of_perm hP]
+
+
+lemma Typing_inv_one {n : Nat} {P : Proc} {x : FPName} {𝒢 : HyperEnv}
+  (hT : Typing n (#x⟦⟧․P) 𝒢) :
+  (𝒢 ~ [[x ∶ 1]]) ∧ Typing n P ∅ := by
+  generalize heq : (#x⟦⟧․P) = P' at hT
+  induction hT generalizing P x <;> try contradiction
+
+  case exchange_env ℋ _ _ _ _ _ hP ih =>
+    have ⟨h1, h2⟩ := ih heq
+    have := HyperEnv.Perm.cons hP.symm (HyperEnv.Perm.refl ℋ)
+    exact ⟨HyperEnv.Perm.trans this h1, h2⟩
+
+  case exchange_hyper hP ih =>
+    have ⟨h1, h2⟩ := ih heq
+    exact ⟨HyperEnv.Perm.trans hP.symm h1, h2⟩
+
+  case one hT _ =>
+    simp at heq
+    constructor
+    · simp [heq.1, HasPerm.perm]
+    · simp [heq.2]
+      exact hT
+
+lemma Typing_inv_bot {n : Nat} {P : Proc} {x : FPName} {𝒢 : HyperEnv}
+  (hT : Typing n (#x⸨⸩․P) 𝒢) :
+  ∃ Γ, (𝒢 ~ [x ∶ ⊥ :: Γ]) ∧ Typing n P [Γ] := by
+  generalize heq : (#x⸨⸩․P) = P' at hT
+  induction hT generalizing P x <;> try contradiction
+
+  case exchange_env ℋ _ _ _ _ _ hP ih =>
+    have ⟨Ξ, h⟩ := ih heq
+    obtain ⟨h1, h2⟩ := h
+    constructor
+    · have := HyperEnv.Perm.cons hP.symm (HyperEnv.Perm.refl ℋ)
+      exact ⟨HyperEnv.Perm.trans this h1, h2⟩
+
+  case exchange_hyper hP ih =>
+    have ⟨Γ, h⟩ := ih heq
+    obtain ⟨h1, h2⟩ := h
+    constructor
+    · exact ⟨HyperEnv.Perm.trans hP.symm h1, h2⟩
+
+  case bot hT _ =>
+    simp at heq
+    constructor
+    · constructor
+      · simp [heq.1]
+        apply HyperEnv.Perm.refl
+      · simp [heq.2]
+        exact hT
+
+lemma Typing_inv_tensor {n : Nat} {P : Proc} {𝒢 : HyperEnv} {x : FPName}
+  (hT : Typing n (#x⟦$N⟧․P) 𝒢) :
+  ∃ (A B : Types) (Γ Δ : Env) (L : Finset FPName),
+    (𝒢 ~ [x ∶ A ⨂ B :: Γ‚ Δ]) ∧ (∀ z ∉ L, Typing n (P⸨#z⸩) ([z ∶ A :: Γ] |ₕ [x ∶ B :: Δ])) := by
+  generalize heq : (#x⟦$N⟧․P) = P' at hT
+  induction hT generalizing P <;> try contradiction
+
+  case exchange_env hP ih =>
+    obtain ⟨A, B, Γ, Δ, L, hP', hT'⟩ := ih heq
+    use A, B, Γ, Δ, L
+    constructor
+    · exact (HyperEnv.Perm.trans (hP'.symm) (HyperEnv.Perm.cons hP (HyperEnv.Perm.refl _))).symm
+    · exact hT'
+
+  case exchange_hyper hP ih =>
+    obtain ⟨A, B, Γ, Δ, L, hP', hT'⟩ := ih heq
+    use A, B, Γ, Δ, L
+    constructor
+    · exact HyperEnv.Perm.trans (hP.symm) hP'
+    · exact hT'
+
+  case tensor Γ Δ Q _ A B _ _ L hT ih =>
+    obtain ⟨z, hz⟩ := exists_one_fresh (L ∪ Γ.names ∪ Δ.names ∪ Q.f ∪ {x})
+    simp at hz heq
+    obtain ⟨hz1, hz2, hz3, hz4, hz5⟩ := hz
+    use A, B, Γ, Δ, L
+    constructor
+    · rw [heq.1]
+    · rw [heq.1, heq.2]
+      exact hT
+
+lemma Typing_inv_parr {n : Nat} {P : Proc} {𝒢 : HyperEnv} {x : FPName}
+  (hT : Typing n (#x⸨$N⸩․P) 𝒢) :
+  ∃ (A B : Types) (Γ : Env) (L : Finset FPName),
+    (𝒢 ~ [x ∶ A ⅋ B :: Γ]) ∧ (∀ z ∉ L, Typing n (P⸨#z⸩) ([z ∶ A :: x ∶ B :: Γ])) := by
+  generalize heq : (#x⸨$N⸩․P) = P' at hT
+  induction hT generalizing P <;> try contradiction
+
+  case exchange_env hP ih =>
+    obtain ⟨A, B, Γ, L, hP', hT'⟩:= ih heq
+    use A, B, Γ, L
+    constructor
+    · exact (HyperEnv.Perm.trans (hP'.symm) (HyperEnv.Perm.cons hP (HyperEnv.Perm.refl _))).symm
+    · exact hT'
+
+  case exchange_hyper hP ih =>
+    obtain ⟨A, B, Γ, L, hP', hT'⟩ := ih heq
+    use A, B, Γ, L
+    constructor
+    · exact HyperEnv.Perm.trans (hP.symm) hP'
+    · exact hT'
+
+  case parr Γ Q y A B hF n L hT ih =>
+    obtain ⟨z, hz⟩ := exists_one_fresh (L ∪ Γ.names ∪ Q.f ∪ {x})
+    simp at hz heq
+    obtain ⟨hz1, hz2, hz3, hz4⟩ := hz
+    use A, B, Γ, L
+    constructor
+    · rw [heq.1]
+    · rw [heq.1, heq.2]
+      exact hT
+
+lemma Typing_inv_par {n : Nat} {P Q : Proc} {𝒢 : HyperEnv} (hT : n ⊢ P |ₚ Q ∷ 𝒢) :
+  ∃ 𝒢₁ 𝒢₂, (𝒢 ~ 𝒢₁ |ₕ 𝒢₂) ∧ (n ⊢ P ∷ 𝒢₁) ∧ (n ⊢ Q ∷ 𝒢₂) := by
+  generalize heq : (P |ₚ Q) = PQ at hT
+  induction hT generalizing P Q <;> try contradiction
+
+  case exchange_env hP ih =>
+    obtain ⟨ℋ₁, ℋ₂, hP', hT'⟩ := ih heq
+    use ℋ₁, ℋ₂
+    constructor
+    · exact HyperEnv.Perm.trans (HyperEnv.Perm.cons hP.symm (HyperEnv.Perm.refl _)) hP'
+    · exact hT'
+
+  case exchange_hyper hP ih =>
+    obtain ⟨ℋ₁, ℋ₂, hP', hT'⟩ := ih heq
+    use ℋ₁, ℋ₂
+    constructor
+    · exact HyperEnv.Perm.trans hP.symm hP'
+    · exact hT'
+
+  case mix 𝒢 ℋ _ _ hD _ hTP hTQ ihP ihQ =>
+    simp at heq
+    obtain ⟨hP, hQ⟩ := heq
+    use 𝒢, ℋ
+    rw [hP, hQ]
+    exact ⟨by simp, ⟨hTP, hTQ⟩⟩
+
+lemma Typing_inv_link {n : Nat} {x y : FPName} {𝒢 : HyperEnv}
+  (hT : n ⊢ #x⟷ₚ#y ∷ 𝒢) :
+  ∃ A, 𝒢 ~ [x ∶ Aᗮ :: [y ∶ A]] := by
+  generalize heq : (#x⟷ₚ#y) = P at hT
+  induction hT generalizing x y <;> try contradiction
+
+  case exchange_env hP ih =>
+    obtain ⟨T, hP'⟩ := ih heq
+    use T
+    exact HyperEnv.Perm.trans (HyperEnv.Perm.cons hP.symm HyperEnv.Perm.rfl) hP'
+
+  case exchange_hyper hP ih =>
+    obtain ⟨T, hP'⟩ := ih heq
+    use T
+    exact HyperEnv.Perm.trans hP.symm hP'
+
+  case ax A _ hneq hlc =>
+    simp at heq
+    obtain ⟨rfl, rfl⟩ := heq
+    use A
+
+lemma Typing_inv_amp {n : Nat} {x : FPName} {P Q : Proc} {𝒢 : HyperEnv}
+  (hT : n ⊢ #x․case{𝐋 : P, 𝐑 : Q} ∷ 𝒢) :
+  ∃ Γ A B, (𝒢 ~ [x ∶ A & B :: Γ]) ∧ (n ⊢ P ∷ [x ∶ A :: Γ]) ∧ (n ⊢ Q ∷ [x ∶ B :: Γ]) := by
+  generalize heq : (#x․case{𝐋 : P, 𝐑 : Q}) = PQ at hT
+  induction hT generalizing P Q x <;> try contradiction
+
+  case exchange_env hP ih =>
+    obtain ⟨𝒢', A, B, hP', hT'⟩ := ih heq
+    use 𝒢', A, B
+    constructor
+    · exact HyperEnv.Perm.trans (HyperEnv.Perm.cons hP.symm (HyperEnv.Perm.refl _)) hP'
+    · exact hT'
+
+  case exchange_hyper hP ih =>
+    obtain ⟨𝒢', A, B, hP', hT'⟩ := ih heq
+    use 𝒢', A, B
+    constructor
+    · exact HyperEnv.Perm.trans hP.symm hP'
+    · exact hT'
+
+  case amp Γ _ _ x A B _ hTP hTQ ihP ihQ =>
+    simp at heq
+    obtain ⟨rfl, rfl, rfl⟩ := heq
+    use Γ, A, B
+
+lemma Typing_inv_selectL {n : Nat} {x : FPName} {P : Proc} {𝒢 : HyperEnv}
+  (hT : n ⊢ #x⟦𝐋⟧․P ∷ 𝒢) :
+  ∃ Γ A B, (𝒢 ~ [x ∶ A ⊕ B :: Γ]) ∧ (n ⊢ P ∷ [x ∶ A :: Γ]) := by
+  generalize heq : (#x⟦𝐋⟧․P) = PsL at hT
+  induction hT generalizing P x <;> try contradiction
+
+  case exchange_env hP ih =>
+    obtain ⟨Γ, A, B, hP', hT'⟩ := ih heq
+    use Γ, A, B
+    constructor
+    · exact HyperEnv.Perm.trans (HyperEnv.Perm.cons hP.symm (HyperEnv.Perm.refl _)) hP'
+    · exact hT'
+
+  case exchange_hyper hP ih =>
+    obtain ⟨Γ, A, B, hP', hT'⟩ := ih heq
+    use Γ, A, B
+    constructor
+    · exact HyperEnv.Perm.trans hP.symm hP'
+    · exact hT'
+
+  case oplus₁ Γ _ _ A B  _ hlc hPT ih =>
+    simp at heq
+    obtain ⟨rfl, rfl⟩ := heq
+    use Γ, A, B
+
+lemma Typing_inv_selectR {n : Nat} {x : FPName} {P : Proc} {𝒢 : HyperEnv}
+  (hT : n ⊢ #x⟦𝐑⟧․P ∷ 𝒢) :
+  ∃ Γ A B, (𝒢 ~ [x ∶ A ⊕ B :: Γ]) ∧ (n ⊢ P ∷ [x ∶ B :: Γ]) := by
+  generalize heq : (#x⟦𝐑⟧․P) = PsR at hT
+  induction hT generalizing P x <;> try contradiction
+
+  case exchange_env hP ih =>
+    obtain ⟨Γ, A, B, hP', hT'⟩ := ih heq
+    use Γ, A, B
+    constructor
+    · exact HyperEnv.Perm.trans (HyperEnv.Perm.cons hP.symm (HyperEnv.Perm.refl _)) hP'
+    · exact hT'
+
+  case exchange_hyper hP ih =>
+    obtain ⟨Γ, A, B, hP', hT'⟩ := ih heq
+    use Γ, A, B
+    constructor
+    · exact HyperEnv.Perm.trans hP.symm hP'
+    · exact hT'
+
+  case oplus₂ Γ _ _ A B  _ hlc hPT ih =>
+    simp at heq
+    obtain ⟨rfl, rfl⟩ := heq
+    use Γ, A, B
+
+lemma Typing_inv_output {n : Nat} {x : FPName} {A : Types} {P : Proc} {𝒢 : HyperEnv}
+  (hT : n ⊢ #x⟦A⟧․P ∷ 𝒢) :
+  ∃ Γ B,
+  (𝒢 ~ [x ∶ ∃․B :: Γ]) ∧ n ⊢ P ∷ [x ∶ B{A // 0} :: Γ] := by
+  generalize heq : (#x⟦A⟧․P) = Pout at hT
+  induction hT generalizing P x <;> try contradiction
+
+  case exchange_env hP ih =>
+    obtain ⟨Γ, B, hP', hT'⟩ := ih heq
+    use Γ, B
+    constructor
+    · exact HyperEnv.Perm.trans (HyperEnv.Perm.cons hP.symm (HyperEnv.Perm.refl _)) hP'
+    · exact hT'
+
+  case exchange_hyper hP ih =>
+    obtain ⟨Γ, A, hP', hT'⟩ := ih heq
+    use Γ, A
+    constructor
+    · exact HyperEnv.Perm.trans hP.symm hP'
+    · exact hT'
+
+  case exists_ Γ _ _ _ B _ hlc hT ih =>
+    simp at heq
+    obtain ⟨rfl, rfl, rfl⟩ := heq
+    use Γ, B
+
+lemma Typing_inv_input {n : Nat} {x : FPName} {P : Proc} {𝒢 : HyperEnv}
+  (hT : n ⊢ #x⸨$T⸩․P ∷ 𝒢) :
+  ∃ (Γ : Env) (B : Types),
+  (𝒢 ~ [x ∶ ∀․B :: Γ]) ∧ (n + 1 ⊢ P ∷ [x ∶ B :: Γ⁺ᵗ]) := by
+  generalize heq : (#x⸨$T⸩․P) = Pin at hT
+  induction hT generalizing P x <;> try contradiction
+
+  case exchange_env hP ih =>
+    obtain ⟨Γ, B, hP', hT'⟩ := ih heq
+    use Γ, B
+    constructor
+    · exact HyperEnv.Perm.trans (HyperEnv.Perm.cons hP.symm (HyperEnv.Perm.refl _)) hP'
+    · exact hT'
+
+  case exchange_hyper hP ih =>
+    obtain ⟨Γ, B, hP', hT'⟩ := ih heq
+    use Γ, B
+    constructor
+    · exact HyperEnv.Perm.trans hP.symm hP'
+    · exact hT'
+
+  case forall_ Γ _ _ B _ _ ih  =>
+    simp at heq
+    obtain ⟨rfl, rfl⟩ := heq
+    use Γ, B
+
+lemma Typing_inv_use₁ {n : Nat} {x : FPName} {P : Proc} {𝒢 : HyperEnv}
+  (hT : n ⊢ #x⟦USE⟧․P ∷ 𝒢) :
+  ∃ Γ A, (𝒢 ~ [x ∶ ??A :: Γ]) ∧ (n ⊢ P ∷ [x ∶ A :: Γ]) := by
+  generalize heq : (#x⟦USE⟧․P) = Puse at hT
+  induction hT generalizing P x <;> try contradiction
+
+  case exchange_env 𝒢 _ _ _ _ _ hP ih =>
+    obtain ⟨Γ, A, hP', hT'⟩ := ih heq
+    use Γ, A
+    constructor
+    · exact HyperEnv.Perm.trans (HyperEnv.Perm.cons hP.symm (HyperEnv.Perm.refl 𝒢)) hP'
+    · exact hT'
+
+  case exchange_hyper hP ih =>
+    obtain ⟨Γ, A, hP', hT'⟩ := ih heq
+    use Γ, A
+    constructor
+    · exact HyperEnv.Perm.trans hP.symm hP'
+    · exact hT'
+
+  case quest Γ _ _ A _ _ ih =>
+    simp at heq
+    obtain ⟨rfl, rfl⟩ := heq
+    use Γ, A
+
+lemma Typing_inv_use₂ {n : Nat} {x : FPName} {P : Proc} {𝒢 : HyperEnv}
+  (hT : n ⊢ !#x․{P} ∷ 𝒢) :
+  ∃ Γ A, (𝒢 ~ [x ∶ !!A :: Γ]) ∧ (n ⊢ P ∷ [x ∶ A :: Γ]) ∧ ?ₑΓ := by
+  generalize heq : (!#x․{P}) = Puse at hT
+  induction hT generalizing P x <;> try contradiction
+
+  case exchange_env 𝒢 _ _ _ _ _ hP ih =>
+    obtain ⟨Γ, A, hP', hT'⟩ := ih heq
+    use Γ, A
+    constructor
+    · exact HyperEnv.Perm.trans (HyperEnv.Perm.cons hP.symm (HyperEnv.Perm.refl 𝒢)) hP'
+    · exact hT'
+
+  case exchange_hyper hP ih =>
+    obtain ⟨Γ, A, hP', hT'⟩ := ih heq
+    use Γ, A
+    constructor
+    · exact HyperEnv.Perm.trans hP.symm hP'
+    · exact hT'
+
+  case bang Γ _ _ A _ _ _ _ =>
+    simp at heq
+    obtain ⟨rfl, rfl⟩ := heq
+    use Γ, A
+
+lemma Typing_inv_disp₁ {n : Nat} {x : FPName} {P : Proc} {𝒢 : HyperEnv}
+  (hT : n ⊢ #x⟦DISP⟧․P ∷ 𝒢) :
+  ∃ Γ A, (𝒢 ~ [x ∶ ??A :: Γ]) ∧ (n ⊢ P ∷ [Γ]) ∧ x ∉ Env.names Γ := by
+  generalize heq : (#x⟦DISP⟧․P) = Pdisp at hT
+  induction hT generalizing P x <;> try contradiction
+
+  case exchange_env hP ih =>
+    obtain ⟨Γ, A, hP', hT'⟩ := ih heq
+    use Γ, A
+    constructor
+    · exact HyperEnv.Perm.trans (HyperEnv.Perm.cons hP.symm (HyperEnv.Perm.refl _)) hP'
+    · exact hT'
+
+  case exchange_hyper hP ih =>
+    obtain ⟨Γ, A, hP', hT'⟩ := ih heq
+    use Γ, A
+    constructor
+    · exact HyperEnv.Perm.trans hP.symm hP'
+    · exact hT'
+
+  case w Γ _ _ A _ _ _ _ _ =>
+    simp at heq
+    obtain ⟨rfl, rfl⟩ := heq
+    use Γ, A
+
+lemma Typing_inv_dup₁ {n : Nat} {x : FPName} {P : Proc} {𝒢 : HyperEnv}
+  (hT : n ⊢ #x⟦DUP⟧⸨$N⸩․P ∷ 𝒢) :
+  ∃ (Γ : Env) (A : Types) (L : Finset FPName),
+    (𝒢 ~ [x ∶ ??A :: Γ]) ∧ x ∉ Γ.names ∧
+    (∀ x' ∉ L, x' ≠ x → n ⊢ P⸨#x'⸩ ∷ [x' ∶ ??A :: x ∶ ??A :: Γ]) := by
+  generalize heq : (#x⟦DUP⟧⸨$N⸩․P) = Pdup at hT
+  induction hT generalizing P x <;> try contradiction
+
+  case exchange_env hP ih =>
+    obtain ⟨Γ, A, x', hP', hT'⟩ := ih heq
+    use Γ, A, x'
+    constructor
+    · exact HyperEnv.Perm.trans (HyperEnv.Perm.cons hP.symm (HyperEnv.Perm.refl _)) hP'
+    · exact hT'
+
+  case exchange_hyper hP ih =>
+    obtain ⟨Γ, A, x', hP', hT'⟩ := ih heq
+    use Γ, A, x'
+    constructor
+    · exact HyperEnv.Perm.trans hP.symm hP'
+    · exact hT'
+
+  case c Γ _ _ A _ hF L hT _ =>
+    simp at heq
+    obtain ⟨rfl, rfl⟩ := heq
+    use Γ, A, L
+    constructor
+    · simp
+    · constructor
+      · exact hF
+      · intros x' hin hneq
+        apply Typing.exchange_hyper (hT x' hin)
+        exact HyperEnv.Perm.cons (List.Perm.swap (x' ∶ ??A) (x ∶ ??A) Γ) (by simp)
+
+lemma Typing_inv_res {n : ℕ} {P : Proc} {𝒢 : HyperEnv}
+  (hT : n ⊢ 𝑣⸨$N,$N⸩ P ∷ 𝒢) :
+  ∃ (A : Types) (Γ Δ : Env) (𝒢' : HyperEnv) (L : Finset FPName),
+    (𝒢 ~ 𝒢' |ₕ [Γ‚ Δ]) ∧
+    (∀ x ∉ L, ∀ y ∉ L, x ≠ y →
+      n ⊢ P⸨#x, #y⸩ ∷ 𝒢' |ₕ [x ∶ A :: Γ] |ₕ [y ∶ Aᗮ :: Δ]) := by
+
+  generalize heq : (𝑣⸨$N,$N⸩ P) = P' at hT
+  induction hT generalizing P <;> try contradiction
+
+  case exchange_env hP ih =>
+    obtain ⟨A, Γ, Δ, 𝒢, L, hP', hT'⟩ := ih heq
+    use A, Γ, Δ, 𝒢, L
+    constructor
+    · exact HyperEnv.Perm.trans (HyperEnv.Perm.cons hP.symm (by rfl)) hP'
+    · intros x hx y hy hneq
+      exact hT' x hx y hy hneq
+
+  case exchange_hyper hP ih =>
+    obtain ⟨A, Γ, Δ, 𝒢, L, hP', hT'⟩ := ih heq
+    use A, Γ, Δ, 𝒢, L
+    constructor
+    · exact HyperEnv.Perm.trans hP.symm hP'
+    · intros x hx y hy hneq
+      exact hT' x hx y hy hneq
+
+  case cut 𝒢 Γ Δ _ A _ L hT ih =>
+    use A, Γ, Δ, 𝒢, L
+    constructor
+    · rfl
+    · injection heq with heq
+      subst heq
+      intros x hx y hy hneq
+      exact hT x y hx hy hneq
